cogent/examples/wa_connect/WordArray_UpdCCorres.thy
@@ -7,76 +7,17 @@ begin
 
 context WordArray begin
 
-thm abbreviated_type_defs
-(*
-abbreviation "w_val h w \<equiv> values_C (h w)"
-abbreviation "w_len h w \<equiv> SCAST(32 signed \<rightarrow> 32) (len_C (h w))"
-
-abbreviation "w_p s w \<equiv> w_val (heap_WordArray_u32_C s) w"
-abbreviation "w_l s w \<equiv> w_len (heap_WordArray_u32_C s) w"
-
-section "Helper Lemma for Word Array Existence and Validity"
- 
-definition valid_c_wordarray
-  where
-  "valid_c_wordarray s w \<equiv> is_valid_WordArray_u32_C s w \<and> 
-                            (\<forall>i < w_l s w. is_valid_w32 s ((w_p s w) +\<^sub>p uint i)) "
-
-definition valid_cogent_wordarray
-  where
-  "valid_cogent_wordarray \<sigma> s w \<equiv> (\<exists>len arr. len = w_l s w \<and> arr = ptr_val (w_p s w) \<and> 
-                                    \<sigma> (ptr_val w) = option.Some (UAbstract (WAU32 len arr)) \<and> 
-                                   (\<forall>i < len. \<sigma> (arr + 4 * i) = option.Some (UPrim (LU32 (heap_w32 s ((w_p s w) +\<^sub>p uint i))))))"
-
-definition valid_wordarray
-  where
-  "valid_wordarray \<sigma> s w \<equiv> valid_c_wordarray s w \<and> valid_cogent_wordarray \<sigma> s w"
-
-
-lemma well_typed_related_wordarray: "\<And>\<sigma> st x x' a ts s r w.
-       \<lbrakk>(\<sigma>, st) \<in> state_rel; val_rel x (x':: WordArray_u32_C ptr); abs_typing_u a ts\<rbrakk>
-       \<Longrightarrow> valid_wordarray \<sigma> st x'"
-  apply (unfold valid_wordarray_def valid_c_wordarray_def valid_cogent_wordarray_def)
-  apply (clarsimp simp: val_rel_simp)
-  apply (erule u_t_recE)
-  apply (erule u_t_r_consE; clarsimp simp: \<Xi>_def wordarray_put2_0_type_def abbreviatedType1_def)
-  apply (erule u_t_p_absE; clarsimp)
-  apply (clarsimp simp: abs_typing'_def)
-  apply (case_tac a; clarsimp)
-  apply (clarsimp simp: state_rel_def heap_rel_def heap_rel_ptr_meta heap_rel_ptr_w32_meta)
-  apply (drule_tac p = "arr_C x'" and uv = "UAbstract (WAU32 x11 x12)" in all_heap_rel_ptrD; 
-         clarsimp simp: type_rel_simp abs_repr'_def val_rel_simp is_valid_simp heap_simp)
-  apply (rule conjI)
-   apply clarsimp
-   apply (erule_tac x = i in allE)
-   apply (erule_tac x = i in allE)
-   apply clarsimp
-   apply (drule_tac uv = "UPrim (LU32 x)" and 
-                     p = "values_C (heap_WordArray_u32_C st (arr_C x')) +\<^sub>p uint i"
-                     in all_heap_rel_ptrD;
-          clarsimp simp: ptr_add_def mult.commute type_rel_simp)
-  apply clarsimp
-  apply (erule_tac x = i in allE)
-  apply (erule_tac x = i in allE)
-  apply clarsimp
-  apply (drule_tac uv = "UPrim (LU32 x)" and 
-                    p = "values_C (heap_WordArray_u32_C st (arr_C x')) +\<^sub>p uint i"
-                    in all_heap_rel_ptrD;
-         clarsimp simp: ptr_add_def mult.commute type_rel_simp val_rel_simp)
-  done
-*)
-
 section "Correspondence Lemmas Between Update Semantics and C"
 
-declare \<xi>0.simps[simp del]
-lemma upd_C_wordarray_put2_corres:
+lemma upd_C_wordarray_put2_corres_gen:
   "\<And>i \<gamma> v' \<Gamma>' \<sigma> st.
-    \<lbrakk>i < length \<gamma>; val_rel (\<gamma> ! i) v'; \<Gamma>' ! i = option.Some (prod.fst (prod.snd (\<Xi> ''wordarray_put2_0'')))\<rbrakk>
+    \<lbrakk>i < length \<gamma>; val_rel (\<gamma> ! i) v'; \<Gamma>' ! i = option.Some (prod.fst (prod.snd (\<Xi> ''wordarray_put2_0'')));
+     \<xi>0' ''wordarray_put2_0'' = upd_wa_put2_0\<rbrakk>
     \<Longrightarrow> update_sem_init.corres wa_abs_typing_u wa_abs_repr (Generated.state_rel wa_abs_repr) (App (AFun ''wordarray_put2_0'' []) (Var i))
          (do x <- main_pp_inferred.wordarray_put2_0' v';
              gets (\<lambda>s. x)
           od)
-         \<xi>0 \<gamma> \<Xi> \<Gamma>' \<sigma> st"
+         \<xi>0' \<gamma> \<Xi> \<Gamma>' \<sigma> st"
   apply (rule absfun_corres; simp?)
   apply (thin_tac "\<Gamma>' ! i = _")
   apply (clarsimp simp: abs_fun_rel_def; rename_tac r w)
@@ -102,7 +43,7 @@ lemma upd_C_wordarray_put2_corres:
    apply (erule_tac x = "t2_C.idx_C v'" in allE)+
    apply (clarsimp simp: val_rel_simp heap_simp type_rel_simp)
   apply clarsimp
-  apply (monad_eq simp: upd_wa_put2_0_def \<xi>0.simps)
+  apply (monad_eq simp: upd_wa_put2_0_def)
   apply (case_tac "idx_C v' < len"; clarsimp)
   apply (rule conjI)
     apply (monad_eq simp: wordarray_put2_0'_def)
@@ -136,14 +77,17 @@ lemma upd_C_wordarray_put2_corres:
   apply (clarsimp simp: val_rel_simp heap_simp is_valid_simp)
   done
 
-lemma upd_C_wordarray_length_corres:
+lemmas upd_C_wordarray_put2_corres = upd_C_wordarray_put2_corres_gen[rotated -1, of \<xi>0, simplified fun_eq_iff]
+
+lemma upd_C_wordarray_length_corres_gen:
 "\<And>i \<gamma> v' \<Gamma>' \<sigma> st.
-    \<lbrakk>i < length \<gamma>; val_rel (\<gamma> ! i) v'; \<Gamma>' ! i = option.Some (prod.fst (prod.snd (\<Xi> ''wordarray_length_0'')))\<rbrakk>
+    \<lbrakk>i < length \<gamma>; val_rel (\<gamma> ! i) v'; \<Gamma>' ! i = option.Some (prod.fst (prod.snd (\<Xi> ''wordarray_length_0'')));
+     \<xi>0' ''wordarray_length_0''= upd_wa_length_0\<rbrakk>
     \<Longrightarrow> update_sem_init.corres wa_abs_typing_u wa_abs_repr (Generated.state_rel wa_abs_repr) (App (AFun ''wordarray_length_0'' []) (Var i))
          (do x <- main_pp_inferred.wordarray_length_0' v';
              gets (\<lambda>s. x)
           od)
-         \<xi>0 \<gamma> \<Xi> \<Gamma>' \<sigma> st"
+         \<xi>0' \<gamma> \<Xi> \<Gamma>' \<sigma> st"
   apply (rule absfun_corres; simp?)
   apply (clarsimp simp: abs_fun_rel_def; rename_tac r w)
   apply (thin_tac "\<Gamma>' ! i = _")
@@ -161,7 +105,7 @@ lemma upd_C_wordarray_length_corres:
   apply clarsimp
   apply (rule_tac x = \<sigma> in exI)
   apply (rule conjI)
-   apply (clarsimp simp: upd_wa_length_0_def \<xi>0.simps)
+   apply (clarsimp simp: upd_wa_length_0_def)
    apply (monad_eq simp: wordarray_length_0'_def)
    apply (clarsimp simp: state_rel_def heap_rel_def)
    apply (erule_tac x = v' in allE)
@@ -169,15 +113,17 @@ lemma upd_C_wordarray_length_corres:
   apply (monad_eq simp: wordarray_length_0'_def)
   done
 
+lemmas upd_C_wordarray_length_corres = upd_C_wordarray_length_corres_gen[rotated -1, of \<xi>0, simplified fun_eq_iff]
 
-lemma upd_C_wordarray_get_corres:
+lemma upd_C_wordarray_get_corres_gen:
 "\<And>i \<gamma> v' \<Gamma>' \<sigma> st.
-    \<lbrakk>i < length \<gamma>; val_rel (\<gamma> ! i) v'; \<Gamma>' ! i = option.Some (prod.fst (prod.snd (\<Xi> ''wordarray_get_0'')))\<rbrakk>
+    \<lbrakk>i < length \<gamma>; val_rel (\<gamma> ! i) v'; \<Gamma>' ! i = option.Some (prod.fst (prod.snd (\<Xi> ''wordarray_get_0'')));
+     \<xi>0' ''wordarray_get_0'' = upd_wa_get_0\<rbrakk>
     \<Longrightarrow> update_sem_init.corres wa_abs_typing_u wa_abs_repr (Generated.state_rel wa_abs_repr) (App (AFun ''wordarray_get_0'' []) (Var i))
          (do x <- main_pp_inferred.wordarray_get_0' v';
              gets (\<lambda>s. x)
           od)
-         \<xi>0 \<gamma> \<Xi> \<Gamma>' \<sigma> st"
+         \<xi>0' \<gamma> \<Xi> \<Gamma>' \<sigma> st"
   apply (rule absfun_corres; simp?)
   apply (clarsimp simp: abs_fun_rel_def; rename_tac r w)
   apply (thin_tac "\<Gamma>' ! i = _")
@@ -204,7 +150,7 @@ lemma upd_C_wordarray_get_corres:
   apply clarsimp
   apply (rule_tac x = \<sigma> in exI)
   apply (rule conjI)
-   apply (clarsimp simp: upd_wa_get_0_def \<xi>0.simps)
+   apply (clarsimp simp: upd_wa_get_0_def)
    apply (frule wa_abs_typing_u_elims(5))
    apply (erule_tac x = "t1_C.p2_C v'" in allE)
    apply (monad_eq simp: wordarray_get_0'_def word_less_nat_alt word_le_nat_alt)
@@ -217,590 +163,8 @@ lemma upd_C_wordarray_get_corres:
   apply (monad_eq simp: wordarray_get_0'_def)
   apply blast
   done
-thm corres_sum corres_app_concrete
-declare \<xi>1.simps [simp del]
-(*
-lemma upd_C_wordarray_fold_no_break_corres:
-" \<And>v' i \<gamma> \<Gamma>' \<sigma> s.
-    \<lbrakk>i < length \<gamma>; val_rel (\<gamma> ! i) v';
-     \<Gamma>' ! i = option.Some (prod.fst (prod.snd (\<Xi> ''wordarray_fold_no_break_0'')))\<rbrakk>
-    \<Longrightarrow> update_sem_init.corres wa_abs_typing_u wa_abs_repr (Generated.state_rel wa_abs_repr)
-         (App (AFun ''wordarray_fold_no_break_0'' []) (Var i)) (do x <- main_pp_inferred.wordarray_fold_no_break_0' v';
-gets (\<lambda>s. x)
-                                                                od)
-         \<xi>1 \<gamma> \<Xi>  \<Gamma>' \<sigma> s"
-  apply (rule absfun_corres; simp?)
-  apply (clarsimp simp: abs_fun_rel_def')
-  apply (thin_tac "\<Gamma>' ! i = _")
-  apply clarsimp
-  apply (clarsimp simp: val_rel_simp)
-  apply (erule upd.u_t_recE)
-  apply (rotate_tac -3)
-  apply (subst (asm) \<Xi>_def)
-  apply (clarsimp simp: wordarray_fold_no_break_0_type_def abbreviated_type_defs)
-  apply (erule upd.u_t_r_consE; clarsimp)+
-  apply (erule upd.u_t_primE; subst (asm) lit_type.simps; clarsimp)+
-  apply (erule upd.u_t_r_emptyE)
-  apply (erule upd.u_t_unitE)
-  apply (case_tac "sint (t5_C.f_C v') \<noteq> sint FUN_ENUM_mul \<and> sint (t5_C.f_C v') \<noteq> sint FUN_ENUM_sum")
-   apply (clarsimp simp: cogent_function_val_rel
-                         FUN_ENUM_sum_def
-                         FUN_ENUM_mul_def
-                         FUN_ENUM_mul_arr_def
-                         FUN_ENUM_sum_arr_def
-                         FUN_ENUM_wordarray_get_0_def
-                         FUN_ENUM_wordarray_length_0_def
-                         FUN_ENUM_wordarray_put2_0_def
-                         FUN_ENUM_wordarray_fold_no_break_0_def
-                         FUN_ENUM_wordarray_get_u32_def
-                         FUN_ENUM_wordarray_length_u32_def
-                         FUN_ENUM_wordarray_put2_u32_def)
-   apply (rule FalseE) 
-   apply (thin_tac "_ \<in> state_rel")
-   apply (thin_tac "t5_C.f_C v' \<noteq> 0")
-   apply (thin_tac "sint (t5_C.f_C v') \<noteq> 2")
-   apply (thin_tac "upd.uval_typing _ _ (UPtr _ _) _ _ _")
-   apply (thin_tac "_ = _")+
-   apply clarsimp
-   apply (erule disjE)
-    prefer 2
-    apply (erule disjE)
-     prefer 2
-     apply (erule disjE)
-      apply clarsimp
-      apply (erule upd.u_t_afunE; clarsimp)
-      apply (clarsimp simp: subtyping_simps(4) 
-                            subtyping.simps[of _ _ "TPrim (Num U32)", simplified]
-                            wordarray_get_0_type_def abbreviated_type_defs
-                            subtyping_simps(6) \<Xi>_def)
-     apply (erule disjE)
-      apply clarsimp
-      apply (erule upd.u_t_afunE; clarsimp)
-      apply (clarsimp simp: subtyping_simps(4) 
-                            subtyping.simps[of _ _ "TPrim (Num U32)", simplified]
-                            wordarray_put2_0_type_def \<Xi>_def)
-     apply (erule disjE)
-      apply clarsimp
-      apply (erule upd.u_t_funE'; clarsimp)
-      apply (clarsimp simp: subtyping_simps(4)
-                            subtyping.simps[of _ "TRecord _ _ ", simplified]
-                            subtyping.simps[of _ _ "TPrim (Num U32)", simplified]
-                            subtyping.simps[of _ "TPrim (Num U32)", simplified]
-                            subtyping.simps[of _ "TUnit", simplified]
-                            kinding_simps(5, 9))
-      apply (clarsimp simp: wordarray_get_u32_def)
-      apply (erule typing_letE)
-      apply (erule typing_appE)
-      apply (erule typing_afunE)
-      apply (clarsimp simp: wordarray_get_0_type_def abbreviated_type_defs \<Xi>_def)
-      apply (erule typing_varE)+
-      apply (clarsimp simp: split_conv_all_nth weakening_conv_all_nth empty_def)
-      apply (erule_tac x = 0 in allE)+
-      apply (clarsimp simp: weakening_comp.simps split_comp.simps)
-      apply (erule disjE; clarsimp)
-     apply (erule disjE)
-      apply clarsimp
-      apply (erule upd.u_t_afunE; clarsimp)
-      apply (clarsimp simp: subtyping_simps(4) 
-                            subtyping.simps[of _ _ "TPrim (Num U32)", simplified]
-                            subtyping.simps[of _ "TRecord _ _ ", simplified]
-                            wordarray_length_0_type_def \<Xi>_def)
-     apply (erule disjE)
-      apply clarsimp
-      apply (erule upd.u_t_funE'; clarsimp)
-      apply (clarsimp simp: subtyping_simps(4)
-                            subtyping.simps[of _ "TRecord _ _ ", simplified]
-                            subtyping.simps[of _ _ "TPrim (Num U32)", simplified]
-                            subtyping.simps[of _ "TPrim (Num U32)", simplified]
-                            subtyping.simps[of _ "TUnit", simplified]
-                            kinding_simps(5, 9))
-      apply (clarsimp simp: wordarray_put2_u32_def)
-      apply (erule typing_letE)
-      apply (erule typing_appE)
-      apply (erule typing_afunE)
-      apply (clarsimp simp: wordarray_put2_0_type_def abbreviated_type_defs \<Xi>_def)
-     apply (erule disjE)
-      apply clarsimp
-      apply (erule upd.u_t_funE'; clarsimp)
-      apply (clarsimp simp: subtyping_simps(4)
-                            subtyping.simps[of _ "TRecord _ _ ", simplified]
-                            subtyping.simps[of _ _ "TPrim (Num U32)", simplified]
-                            subtyping.simps[of _ "TPrim (Num U32)", simplified]
-                            subtyping.simps[of _ "TUnit", simplified]
-                            kinding_simps(5, 9))
-      apply (clarsimp simp: wordarray_length_u32_def)
-      apply (erule typing_letE)
-      apply (erule typing_appE)
-      apply (erule typing_afunE)
-      apply (clarsimp simp: wordarray_length_0_type_def \<Xi>_def)
-      apply (erule typing_varE)+
-      apply (clarsimp simp: split_conv_all_nth weakening_conv_all_nth empty_def)
-      apply (erule_tac x = 0 in allE)+
-      apply (clarsimp simp: weakening_comp.simps split_comp.simps)
-      apply (erule disjE; clarsimp)
-     apply clarsimp
-     apply (erule upd.u_t_afunE; clarsimp)
-     apply (clarsimp simp: subtyping_simps(4) 
-                           subtyping.simps[of _ _ "TPrim (Num U32)", simplified]
-                           subtyping.simps[of _ "TRecord _ _ ", simplified]
-                           \<Xi>_def wordarray_fold_no_break_0_type_def)
-    apply clarsimp
-    apply (erule upd.u_t_funE')
-    apply (clarsimp simp: subtyping_simps(4) 
-                          subtyping.simps[of _ _ "TPrim (Num U32)", simplified]
-                          subtyping.simps[of _ "TRecord _ _ ", simplified]
-                          subtyping.simps[of _ "TPrim (Num U32)", simplified]
-                          subtyping.simps[of _ "TUnit", simplified]
-                          kinding_simps(5, 9))
-    apply (thin_tac "_ \<or> _")+
-    apply (clarsimp simp: sum_arr_def)
-    apply (erule typing_letE)
-    apply (erule typing_letE)
-    apply (erule typing_varE)
-    apply (thin_tac "_, _, (_ #_) \<turnstile> _ : _")
-    apply (erule typing_appE)
-    apply (erule typing_afunE)
-    apply (erule typing_varE)
-    apply (clarsimp simp: wordarray_length_0_type_def \<Xi>_def)
-    apply (frule split_length; simp)
-    apply (drule same_type_as_weakened; simp?)
-    apply (drule split_preservation_some_left; simp?)
-    apply clarsimp
-    apply (drule same_type_as_weakened; simp?)
-    apply (drule_tac ?\<Gamma>2.0 = \<Gamma>2b in split_preservation_some_right; simp?)
-    apply (drule split_preservation_some_left; simp?)
-    apply clarsimp
-   apply clarsimp
-   apply (erule upd.u_t_funE')
-   apply (clarsimp simp: subtyping_simps(4) 
-                         subtyping.simps[of _ _ "TPrim (Num U32)", simplified]
-                         subtyping.simps[of _ "TRecord _ _ ", simplified]
-                         subtyping.simps[of _ "TPrim (Num U32)", simplified]
-                         subtyping.simps[of _ "TUnit", simplified]
-                         kinding_simps(5, 9))
-   apply (thin_tac "_ \<or> _")+
-   apply (clarsimp simp: mul_arr_def)
-   apply (erule typing_letE)
-   apply (erule typing_letE)
-   apply (erule typing_varE)
-   apply (thin_tac "_, _, (_ #_) \<turnstile> _ : _")
-   apply (erule typing_appE)
-   apply (erule typing_afunE)
-   apply (erule typing_varE)
-   apply (clarsimp simp: wordarray_length_0_type_def \<Xi>_def)
-   apply (frule split_length; simp)
-   apply (drule same_type_as_weakened; simp?)
-   apply (drule split_preservation_some_left; simp?)
-   apply clarsimp
-   apply (drule same_type_as_weakened; simp?)
-   apply (drule_tac ?\<Gamma>2.0 = \<Gamma>2b in split_preservation_some_right; simp?)
-   apply (drule split_preservation_some_left; simp?)
-   apply clarsimp
-  apply clarsimp
-  apply (erule upd.u_t_p_absE; clarsimp)
-  apply (clarsimp simp: wordarray_fold_no_break_0'_def upd_wa_foldnb_def \<xi>1.simps)
-  apply (subst unknown_bind_ignore)+
-  apply clarsimp
-  apply wp 
-      apply (clarsimp simp: split_def unknown_bind_ignore)
-      apply (subst whileLoop_add_inv
-              [where M = "\<lambda>((_, r), _). unat (t5_C.to_C v') - unat r" and 
-                     I = "\<lambda>(a, b) s. 
-                        (\<exists>func. cogent_function_val_rel x (sint (t5_C.f_C v')) \<and> func = x \<and>
-                        is_uval_fun func \<and> (\<Xi>, [], [option.Some abbreviatedType1] \<turnstile> 
-                          (App (uvalfun_to_exprfun func) (Var 0)) : TPrim (Num U32)) \<and>
-                        upd_wa_foldnb_bod \<xi>0 \<sigma> (ptr_val (t5_C.arr_C v')) (t5_C.frm_C v') b 
-                          (uvalfun_to_exprfun func) (UPrim (LU32 (t5_C.acc_C v'))) UUnit {} 
-                          (\<sigma>, UPrim (LU32 (t3_C.acc_C a)))) \<and> 
-                        (\<sigma>, s) \<in> state_rel \<and> t5_C.frm_C v' \<le> b \<and>
-                        ret = min (t5_C.to_C v') ((SCAST(32 signed \<rightarrow> 32))(len_C (heap_WordArray_u32_C s (t5_C.arr_C v')))) \<and>
-                        (t5_C.frm_C v' \<le> ret \<longrightarrow> b \<le> ret) \<and> (t5_C.frm_C v' \<ge> ret \<longrightarrow> b = t5_C.frm_C v')"])
-      apply (wp; clarsimp simp: split_def unknown_bind_ignore)
-           apply (clarsimp simp: split_def dispatch_t4'_def unknown_bind_ignore)
-           apply wp
-            apply (clarsimp simp: mul'_def unknown_bind_ignore)
-            apply wp
-           apply (clarsimp simp: sum'_def unknown_bind_ignore)
-           apply wp
-          apply wp
-         apply wp
-        apply wp
-       apply (clarsimp simp: split_def cogent_function_val_rel
-                             FUN_ENUM_sum_def
-                             FUN_ENUM_mul_def
-                             FUN_ENUM_mul_arr_def
-                             FUN_ENUM_sum_arr_def
-                             FUN_ENUM_wordarray_get_0_def
-                             FUN_ENUM_wordarray_length_0_def
-                             FUN_ENUM_wordarray_put2_0_def
-                             FUN_ENUM_wordarray_fold_no_break_0_def
-                             FUN_ENUM_wordarray_get_u32_def
-                             FUN_ENUM_wordarray_length_u32_def
-                             FUN_ENUM_wordarray_put2_u32_def)
-       apply (thin_tac "upd.uval_typing _ _ _ _ _ _")
-       apply (clarsimp simp: wa_abs_typing_u_def)
-       apply (thin_tac "_ \<in> state_rel")
-       apply (clarsimp split: atyp.splits type.splits prim_type.splits)
-       apply (erule_tac x = b in allE)
-       apply (clarsimp simp: state_rel_def heap_rel_def heap_rel_ptr_meta heap_rel_ptr_w32_meta)
-       apply (drule_tac p = "t5_C.arr_C v'" and uv = "UAbstract (UWA (TPrim (Num U32)) x12 x13)" in all_heap_rel_ptrD; 
-              clarsimp simp: type_rel_simps is_valid_simp heap_simp wa_abs_repr_def val_rel_simps) 
-       apply (drule_tac p = "values_C (heap_WordArray_u32_C sa (t5_C.arr_C v')) +\<^sub>p uint b" and 
-                       uv = "UPrim xa" in all_heap_rel_ptrD; clarsimp simp: type_rel_simps)
-       apply (rule conjI; clarsimp)
-        apply (rule conjI)
-         apply (rule_tac r = "UPrim (LU32 (t3_C.acc_C aa))" and 
-                       len = "(SCAST(32 signed \<rightarrow> 32) (len_C (heap_WordArray_u32_C sa (t5_C.arr_C v'))))" and
-                       arr = "(ptr_val (values_C (heap_WordArray_u32_C sa (t5_C.arr_C v'))))" and
-                         v = "UPrim xa" and \<sigma> = \<sigma> and \<sigma>' = \<sigma> and \<sigma>'' = \<sigma> and ?w1.0 = "{}" and 
-                         ?w2.0 = "{}"
-                       in upd_wa_foldnb_bod_step; simp?)
-           apply clarsimp
-          apply (clarsimp simp: frame_def)
-         apply (rule u_sem_app)
-           apply (rule u_sem_fun)
-          apply (rule u_sem_var)
-         apply (subst mul_def; clarsimp)
-         apply (rule u_sem_take_ub; simp?)
-          apply (rule u_sem_var[where \<gamma> = "[_]" and i = 0, simplified])
-         apply clarsimp
-         apply (rule u_sem_take_ub; simp?)
-          apply (rule u_sem_var[where \<gamma> = "[_, _, _]" and i = 1, simplified])
-         apply clarsimp
-         apply (rule u_sem_take_ub; simp?)
-          apply (rule u_sem_var[where \<gamma> = "[_, _, _, _, _]" and i = 1, simplified])
-         apply clarsimp
-         apply (cut_tac \<xi> = \<xi>0 and 
-                        \<gamma> = "[UUnit, 
-                              URecord [(UPrim xa, RPrim (Num U32)),
-                                 (UPrim (LU32 (t3_C.acc_C aa)), RPrim (Num U32)), (UUnit, RUnit)],
-                              UPrim (LU32 (t3_C.acc_C aa)),
-                              URecord [(UPrim xa, RPrim (Num U32)), 
-                                 (UPrim (LU32 (t3_C.acc_C aa)), RPrim (Num U32)), (UUnit, RUnit)],
-                              UPrim xa,
-                              URecord [(UPrim xa, RPrim (Num U32)),
-                                 (UPrim (LU32 (t3_C.acc_C aa)), RPrim (Num U32)), (UUnit, RUnit)],
-                              URecord [(UPrim xa, RPrim (Num U32)),
-                                 (UPrim (LU32 (t3_C.acc_C aa)), RPrim (Num U32)),
-                                 (UUnit, RUnit)]]" and
-                        \<sigma> = \<sigma> and 
-                       \<sigma>' = \<sigma> and
-                        p = "Times U32" and
-                       as = "[Var 4, Var 2]" in u_sem_prim)
-          apply (rule u_sem_all_cons)
-           apply (rule u_sem_var)
-          apply (rule u_sem_all_cons)
-           apply (rule u_sem_var)
-          apply (rule u_sem_all_empty)
-         apply (clarsimp simp: eval_prim_u_def val_rel_simps)
-        apply (rule conjI)  
-         apply (metis (no_types, hide_lams) max_word_max word_Suc_le word_le_less_eq word_not_le)
-        apply (rule conjI)
-         apply clarsimp
-         apply (metis (no_types, hide_lams) max_word_max word_Suc_le word_not_le)
-        apply (rule conjI)
-         apply (meson min_less_iff_conj word_not_le)
-        apply (metis (no_types, hide_lams) add.commute diff_less_mono2 max_word_max unat_mono word_Suc_le word_le_less_eq word_less_nat_alt word_not_le)
-       apply (rule conjI)
-        apply (rule_tac r = "UPrim (LU32 (t3_C.acc_C aa))" and 
-                      len = "(SCAST(32 signed \<rightarrow> 32) (len_C (heap_WordArray_u32_C sa (t5_C.arr_C v'))))" and
-                      arr = "(ptr_val (values_C (heap_WordArray_u32_C sa (t5_C.arr_C v'))))" and
-                        v = "UPrim xa" and \<sigma> = \<sigma> and \<sigma>' = \<sigma> and \<sigma>'' = \<sigma> and ?w1.0 = "{}" and
-                        ?w2.0 = "{}"
-                      in upd_wa_foldnb_bod_step; simp?)
-          apply clarsimp
-         apply (clarsimp simp: frame_def)
-        apply (rule u_sem_app)
-          apply (rule u_sem_fun)
-         apply (rule u_sem_var)
-        apply (subst sum_def; clarsimp)
-        apply (rule u_sem_take_ub; simp?)
-         apply (rule u_sem_var[where \<gamma> = "[_]" and i = 0, simplified])
-        apply clarsimp
-        apply (rule u_sem_take_ub; simp?)
-         apply (rule u_sem_var[where \<gamma> = "[_, _, _]" and i = 1, simplified])
-        apply clarsimp
-        apply (rule u_sem_take_ub; simp?)
-         apply (rule u_sem_var[where \<gamma> = "[_, _, _, _, _]" and i = 1, simplified])
-        apply clarsimp
-        apply (cut_tac \<xi> = \<xi>0 and 
-                       \<gamma> = "[UUnit, 
-                             URecord [(UPrim xa, RPrim (Num U32)),
-                                (UPrim (LU32 (t3_C.acc_C aa)), RPrim (Num U32)), (UUnit, RUnit)],
-                             UPrim (LU32 (t3_C.acc_C aa)),
-                             URecord [(UPrim xa, RPrim (Num U32)), 
-                                (UPrim (LU32 (t3_C.acc_C aa)), RPrim (Num U32)), (UUnit, RUnit)],
-                             UPrim xa,
-                             URecord [(UPrim xa, RPrim (Num U32)),
-                                (UPrim (LU32 (t3_C.acc_C aa)), RPrim (Num U32)), (UUnit, RUnit)],
-                             URecord [(UPrim xa, RPrim (Num U32)),
-                                (UPrim (LU32 (t3_C.acc_C aa)), RPrim (Num U32)),
-                                (UUnit, RUnit)]]" and
-                       \<sigma> = \<sigma> and 
-                      \<sigma>' = \<sigma> and
-                       p = "Plus U32" and
-                      as = "[Var 4, Var 2]"  in u_sem_prim)
-         apply (rule u_sem_all_cons)
-          apply (rule u_sem_var)
-         apply (rule u_sem_all_cons)
-          apply (rule u_sem_var)
-         apply (rule u_sem_all_empty)
-        apply (clarsimp simp: eval_prim_u_def val_rel_simps)  
-       apply (rule conjI)  
-        apply (metis (no_types, hide_lams) max_word_max word_Suc_le word_le_less_eq word_not_le)
-       apply (rule conjI)
-        apply clarsimp
-        apply (metis (no_types, hide_lams) max_word_max word_Suc_le word_not_le)
-       apply (rule conjI)
-        apply (meson min_less_iff_conj word_not_le)
-       apply (metis (no_types, hide_lams) add.commute diff_less_mono2 max_word_max unat_mono word_Suc_le word_le_less_eq word_less_nat_alt word_not_le)
-      apply (thin_tac "_ \<in> state_rel")
-      apply (clarsimp split: atyp.splits type.splits prim_type.splits simp: wa_abs_typing_u_def)
-      apply (clarsimp simp: state_rel_def heap_rel_def heap_rel_ptr_meta heap_rel_ptr_w32_meta)
-      apply (rule_tac x = \<sigma> in exI; clarsimp?)
-      apply (rule conjI; clarsimp?)
-      apply (drule_tac p = "t5_C.arr_C v'" and uv = "UAbstract (UWA (TPrim (Num U32)) x12 x13)" in all_heap_rel_ptrD; 
-             clarsimp simp: type_rel_simps is_valid_simp heap_simp wa_abs_repr_def val_rel_simps) 
-      apply (thin_tac "cogent_function_val_rel _ _")
-      apply (thin_tac "upd.uval_typing _ _ _ _ _ _")
-      apply (rule_tac x = "TPrim (Num U32)" in exI)
-      apply (rule_tac x = "TUnit" in exI)
-      apply (rule_tac x = "''elem''" in exI)
-      apply (rule_tac x = "''acc''" in exI)
-      apply (rule_tac x = "''obsv''" in exI)
-      apply (rule_tac x = "{}" in exI)
-      apply (rule conjI)
-       apply (rule_tac x = "{}" in exI)
-       apply (rule upd.u_t_prim'; clarsimp)
-      apply (rule_tac x = "{}" in exI; clarsimp)
-      apply (rule conjI)
-       apply (rule upd.u_t_unit)
-      apply (clarsimp simp: \<Xi>_def abbreviatedType1_def wordarray_fold_no_break_0_type_def)
-      apply (case_tac "t5_C.to_C v' = b"; clarsimp?)
-      apply (case_tac "b < t5_C.to_C v'"; clarsimp)
-       apply (case_tac x; clarsimp)
-        apply (drule_tac arr = "ptr_val (values_C (heap_WordArray_u32_C sa (t5_C.arr_C v')))" and 
-                         len = "SCAST(32 signed \<rightarrow> 32) (len_C (heap_WordArray_u32_C sa (t5_C.arr_C v')))" 
-                         in upd_wa_foldnb_bod_to_geq_lenD; simp?)
-        apply (rule_tac arr = "ptr_val (values_C (heap_WordArray_u32_C sa (t5_C.arr_C v')))" and 
-                        len = "SCAST(32 signed \<rightarrow> 32) (len_C (heap_WordArray_u32_C sa (t5_C.arr_C v')))" 
-                        in upd_wa_foldnb_bod_to_geq_len; simp)
-       apply (drule_tac arr = "ptr_val (values_C (heap_WordArray_u32_C sa (t5_C.arr_C v')))" and 
-                        len = "SCAST(32 signed \<rightarrow> 32) (len_C (heap_WordArray_u32_C sa (t5_C.arr_C v')))" 
-                        in upd_wa_foldnb_bod_to_geq_lenD; simp?)
-       apply (rule_tac arr = "ptr_val (values_C (heap_WordArray_u32_C sa (t5_C.arr_C v')))" and 
-                       len = "SCAST(32 signed \<rightarrow> 32) (len_C (heap_WordArray_u32_C sa (t5_C.arr_C v')))" 
-                       in upd_wa_foldnb_bod_to_geq_len; simp)
-      apply (case_tac "min (t5_C.to_C v') (SCAST(32 signed \<rightarrow> 32) (len_C (heap_WordArray_u32_C sa (t5_C.arr_C v')))) \<le> t5_C.frm_C v'")
-       apply clarsimp
-       apply (case_tac x; clarsimp)
-        apply (erule upd_wa_foldnb_bod.elims; clarsimp)
-        apply (clarsimp simp: min_def split: if_splits)
-         apply (subst upd_wa_foldnb_bod.simps; clarsimp)
-        apply (subst upd_wa_foldnb_bod.simps; clarsimp)
-       apply (erule upd_wa_foldnb_bod.elims; clarsimp)
-       apply (clarsimp simp: min_def split: if_splits)
-        apply (subst upd_wa_foldnb_bod.simps; clarsimp)
-       apply (subst upd_wa_foldnb_bod.simps; clarsimp)
-      apply clarsimp
-      apply (rule FalseE)
-      apply (meson min_less_iff_disj not_less word_le_less_eq)
-     apply wp
-    apply wp
-   apply clarsimp
-   apply (subst unknown_def[symmetric])
-   apply (rule validNF_unknown)
-  apply (clarsimp simp: cogent_function_val_rel
-                        FUN_ENUM_sum_def
-                        FUN_ENUM_mul_def
-                        FUN_ENUM_mul_arr_def
-                        FUN_ENUM_sum_arr_def
-                        FUN_ENUM_wordarray_get_0_def
-                        FUN_ENUM_wordarray_length_0_def
-                        FUN_ENUM_wordarray_put2_0_def
-                        FUN_ENUM_wordarray_fold_no_break_0_def
-                        FUN_ENUM_wordarray_get_u32_def
-                        FUN_ENUM_wordarray_length_u32_def
-                        FUN_ENUM_wordarray_put2_u32_def)
-  apply (case_tac x; clarsimp)
-   apply (subst upd_wa_foldnb_bod.simps)
-   apply clarsimp
-   apply (subst upd_wa_foldnb_bod.simps)
-   apply clarsimp
-   apply (clarsimp simp: state_rel_def heap_rel_def heap_rel_ptr_meta wa_abs_typing_u_def)
-   apply (clarsimp split: atyp.splits type.splits prim_type.splits)
-   apply (drule_tac p = "t5_C.arr_C v'" and uv = "UAbstract (UWA (TPrim (Num U32)) x12 x13)" in all_heap_rel_ptrD;
-          clarsimp simp: wa_abs_repr_def type_rel_simps is_valid_simp)
-   apply (thin_tac "upd.uval_typing _ _ _ _ _ _")
-   apply (thin_tac "is_valid_WordArray_u32_C _ _")
-   apply (thin_tac "val_rel _ _")
-   apply (erule disjE; clarsimp)
-    apply (rule conjI; clarsimp)
-     apply (rule conjI)
-      apply (rule_tac x = abbreviatedType1 and 
-        ?\<Gamma>1.0 = "[option.Some abbreviatedType1]" and
-        ?\<Gamma>2.0 = "[option.Some abbreviatedType1]" in typing_app)
-        apply (clarsimp simp: split_Cons split_empty)
-        apply (rule_tac k = "{D, S, E}" in share; simp?)
-        apply (clarsimp simp: abbreviatedType1_def)
-        apply (rule kindingI; clarsimp)
-       apply (rule_tac K' = "[]" and t = "abbreviatedType1" and u = "TPrim (Num U32)" in typing_fun; clarsimp?)
-         apply (cut_tac mul_typecorrect') 
-         apply (clarsimp simp: mul_type_def)
-        apply (clarsimp simp: Cogent.empty_def weakening_Cons weakening_nil)
-        apply (rule_tac k = "{D, S, E}" in drop; simp?)
-        apply (clarsimp simp: abbreviatedType1_def)
-        apply (rule kindingI; clarsimp)
-       apply (clarsimp simp: abbreviatedType1_def)
-      apply (rule typing_var; clarsimp simp: weakening_Cons Cogent.empty_def weakening_nil)
-      apply (rule keep; clarsimp simp: abbreviatedType1_def)
-     apply (metis (no_types, hide_lams) min.strict_order_iff min_def_raw not_less_iff_gr_or_eq)
-    apply (rule conjI)
-     apply (rule_tac x = abbreviatedType1 and 
-        ?\<Gamma>1.0 = "[option.Some abbreviatedType1]" and
-        ?\<Gamma>2.0 = "[option.Some abbreviatedType1]" in typing_app)
-       apply (clarsimp simp: split_Cons split_empty)
-       apply (rule_tac k = "{D, S, E}" in share; simp?)
-       apply (clarsimp simp: abbreviatedType1_def)
-       apply (rule kindingI; clarsimp)
-      apply (rule_tac K' = "[]" and t = "abbreviatedType1" and u = "TPrim (Num U32)" in typing_fun; clarsimp?)
-        apply (cut_tac mul_typecorrect')
-        apply (clarsimp simp: mul_type_def)
-       apply (clarsimp simp: Cogent.empty_def weakening_Cons weakening_nil)
-       apply (rule_tac k = "{D, S, E}" in drop; simp?)
-       apply (clarsimp simp: abbreviatedType1_def)
-       apply (rule kindingI; clarsimp)
-      apply (clarsimp simp: abbreviatedType1_def)
-     apply (rule typing_var; clarsimp simp: weakening_Cons Cogent.empty_def weakening_nil)
-     apply (rule keep; clarsimp simp: abbreviatedType1_def)
-    apply (metis (no_types, hide_lams) min.strict_order_iff min_def_raw not_less_iff_gr_or_eq)
-   apply (erule disjE; clarsimp)
-   apply (rule conjI; clarsimp)
-    apply (rule conjI)
-     apply (rule_tac x = abbreviatedType1 and 
-        ?\<Gamma>1.0 = "[option.Some abbreviatedType1]" and
-        ?\<Gamma>2.0 = "[option.Some abbreviatedType1]" in typing_app)
-       apply (clarsimp simp: split_Cons split_empty)
-       apply (rule_tac k = "{D, S, E}" in share; simp?)
-       apply (clarsimp simp: abbreviatedType1_def)
-       apply (rule kindingI; clarsimp)
-      apply (rule_tac K' = "[]" and t = "abbreviatedType1" and u = "TPrim (Num U32)" in typing_fun; clarsimp?)
-        apply (cut_tac sum_typecorrect') 
-        apply (clarsimp simp: sum_type_def)
-       apply (clarsimp simp: Cogent.empty_def weakening_Cons weakening_nil)
-       apply (rule_tac k = "{D, S, E}" in drop; simp?)
-       apply (clarsimp simp: abbreviatedType1_def)
-       apply (rule kindingI; clarsimp)
-      apply (clarsimp simp: abbreviatedType1_def)
-     apply (rule typing_var; clarsimp simp: weakening_Cons Cogent.empty_def weakening_nil)
-     apply (rule keep; clarsimp simp: abbreviatedType1_def)
-    apply (metis (no_types, hide_lams) min.strict_order_iff min_def_raw not_less_iff_gr_or_eq)
-   apply (rule conjI)
-    apply (rule_tac x = abbreviatedType1 and 
-        ?\<Gamma>1.0 = "[option.Some abbreviatedType1]" and
-        ?\<Gamma>2.0 = "[option.Some abbreviatedType1]" in typing_app)
-      apply (clarsimp simp: split_Cons split_empty)
-      apply (rule_tac k = "{D, S, E}" in share; simp?)
-      apply (clarsimp simp: abbreviatedType1_def)
-      apply (rule kindingI; clarsimp)
-     apply (rule_tac K' = "[]" and t = "abbreviatedType1" and u = "TPrim (Num U32)" in typing_fun; clarsimp?)
-       apply (cut_tac sum_typecorrect')
-       apply (clarsimp simp: sum_type_def)
-      apply (clarsimp simp: Cogent.empty_def weakening_Cons weakening_nil)
-      apply (rule_tac k = "{D, S, E}" in drop; simp?)
-      apply (clarsimp simp: abbreviatedType1_def)
-      apply (rule kindingI; clarsimp)
-     apply (clarsimp simp: abbreviatedType1_def)
-    apply (rule typing_var; clarsimp simp: weakening_Cons Cogent.empty_def weakening_nil)
-    apply (rule keep; clarsimp simp: abbreviatedType1_def)
-   apply (metis (no_types, hide_lams) min.strict_order_iff min_def_raw not_less_iff_gr_or_eq)
-  apply (erule disjE; clarsimp)
-  done
-thm corres_sum corres_app_concrete
 
-lemma 
-" \<And>v' i \<gamma> \<Gamma> \<sigma> s.
-        \<lbrakk>f_C v' = FUN_ENUM_mul; i < length \<gamma>; val_rel (\<gamma> ! i) v';
-         \<Gamma> ! i =
-         option.Some
-          (prod.fst
-            (prod.snd
-              (assoc_lookup
-                [(''wordarray_get_0'', wordarray_get_0_type), (''wordarray_length_0'', wordarray_length_0_type),
-                 (''wordarray_put2_0'', wordarray_put2_0_type), (''wordarray_fold_no_break_0'', wordarray_fold_no_break_0_type),
-                 (''wordarray_get_u32'', Generated_TypeProof.wordarray_get_u32_type),
-                 (''wordarray_length_u32'', Generated_TypeProof.wordarray_length_u32_type),
-                 (''wordarray_put2_u32'', Generated_TypeProof.wordarray_put2_u32_type), (''mul'', Generated_TypeProof.mul_type),
-                 (''mul_arr'', Generated_TypeProof.mul_arr_type), (''sum'', Generated_TypeProof.sum_type),
-                 (''sum_arr'', Generated_TypeProof.sum_arr_type)]
-                ([], TUnit, TUnit) ''wordarray_fold_no_break_0'')))\<rbrakk>
-        \<Longrightarrow> update_sem_init.corres wa_abs_typing_u wa_abs_repr (Generated.state_rel wa_abs_repr)
-             (App (AFun ''wordarray_fold_no_break_0'' []) (Var i)) (do x <- wordarray_fold_no_break_0' v';
-      gets (\<lambda>s. x)
-   od)
-             \<xi>1 \<gamma>
-             (assoc_lookup
-               [(''wordarray_get_0'', wordarray_get_0_type), (''wordarray_length_0'', wordarray_length_0_type),
-                (''wordarray_put2_0'', wordarray_put2_0_type), (''wordarray_fold_no_break_0'', wordarray_fold_no_break_0_type),
-                (''wordarray_get_u32'', Generated_TypeProof.wordarray_get_u32_type),
-                (''wordarray_length_u32'', Generated_TypeProof.wordarray_length_u32_type),
-                (''wordarray_put2_u32'', Generated_TypeProof.wordarray_put2_u32_type), (''mul'', Generated_TypeProof.mul_type),
-                (''mul_arr'', Generated_TypeProof.mul_arr_type), (''sum'', Generated_TypeProof.sum_type),
-                (''sum_arr'', Generated_TypeProof.sum_arr_type)]
-               ([], TUnit, TUnit))
-             \<Gamma> \<sigma> s"
-  
-  by (drule_tac ?\<Gamma>' = \<Gamma> and \<sigma> = \<sigma> and s = s in upd_C_wordarray_fold_no_break_corres[simplified]; simp add: \<Xi>_def)
- *)
-(*
-High level:
-  * Cogent is a language which eases proving things
-    (ASPLOS Paper: we verified Cogent shallow embedding up to a function spec and it was easy)
-  * Can't do everything in Cogent
-    (No iteration or recursion,
-     linear type system enforces restrictions which are too strict sometimes
-        TODO: 
-          Find examples:
-            - vnode pointers in FS file tables esp. if things like dup2 or Linux fork semantic are
-              implemented (i.e. multiple references to the same vnode)
-            -
-          Note here that the C foreign functions  have to respect the type system + frame
-          Easy in C but hard/impossible in Cogent due to linear types but still respects type system and frame
-    ) 
-  * We have an FFI to C
-    (Introduced in ICFP paper with no examples or verification work)
-  * Amortise C verification cost
-    (Intuitive because of ADT reuse, assuming the ssumptions about the C functions are all provable in a reasonable time.
-    Note it is not only the usual correctness assumptions but also frame conditions)
-  * If we verify Cogent bits and verify C bits then the FFI tells us how to put everything together
-    so the entire system is verified
-    (FFI specified some interface which gets you from C all the way up to the shallow embedding
-     The interface we defined was never tested
-     What we did before?
-        Here is a Cogent program that uses a bunch of C. The FFI defines how to compose the Cogent and
-          the C to get an overall proof of correctness. Note however, that this FFI assumes that it
-          has access to a bunch of abstraction functions on types, values, representations, etc, that
-          relate C \<rightarrow> Update \<rightarrow> Value_m \<rightarrow> Value_p \<rightarrow> Shallow and that the abstraction functions respect
-          a bunch of assumptions..
-        Can we actually provide these and discharge the assumptions in order to instantiate the FFI?
-          - abs typing that satisfy locale assumptions
-          - abstractions for abstract values in the update, value and shallow semantics
-          - value relations between C and update, update and value, and value and shallow
-          - abstractions for the abstract functions in the update, value and shallow semantics
-          - proofs for preservation in the update and value semantics for each abstract function
-          - proofs for mono renaming for each abstract function
-          - proofs for correspondence between C and update, update and value, and value and shallow
-          - proofs that the abstraction for the abstract functions in the value semantics execute
-            if the the abstraction for the corresponding abstract function in the update semantics
-            executes
-
-
-
-  * Verified library for word arrays
-      * BilbyFS, Ext2FS
-*)
-thm corres_def corres_app_concrete corres_app_abstract
-thm wordarray_fold_no_break_0'_def hoare_add_K dispatch_t4'_def
+lemmas upd_C_wordarray_get_corres = upd_C_wordarray_get_corres_gen[rotated -1, of \<xi>0, simplified fun_eq_iff]
 
 abbreviation "mk_urecord xs \<equiv> URecord (map (\<lambda>x. (x, upd.uval_repr x)) xs)"
 definition "foldmap_measure i end \<equiv> unat end - unat i"
@@ -809,12 +173,6 @@ definition "foldmap_bounds frm to len i e
 definition "foldmap_inv foldmap \<xi>' \<sigma> p frm i f acc obsv r \<sigma>' res s' res'
   \<equiv> foldmap \<xi>' \<sigma> p frm i f acc obsv r (\<sigma>', res) \<and> val_rel res res' \<and> (\<sigma>', s') \<in> state_rel"
 definition "foldmap_inv_stat obsv obsv' \<equiv> val_rel obsv obsv'"
-lemma state_rel_ex: 
-  "\<exists>\<sigma>. (\<sigma>, s) \<in> state_rel"
-  apply (clarsimp simp: state_rel_def heap_rel_def heap_rel_ptr_def heap_rel_ptr_w32_def)
-  apply (rule_tac x = "\<lambda>_. option.None" in exI)
-  apply clarsimp
-  done
 
 lemma whileLoop_add_invI:
   assumes "\<lbrace> P \<rbrace> whileLoop_inv c b init I (measure M) \<lbrace> Q \<rbrace>!"
@@ -844,10 +202,12 @@ lemma \<Xi>_wordarray_fold_no_break_0:
   "\<Xi> ''wordarray_fold_no_break_0'' = wordarray_fold_no_break_0_type"
   by (clarsimp simp: \<Xi>_def)
 
+abbreviation "elem_type x \<equiv> (present_type \<circ> (\<lambda>xs. xs ! 0) \<circ> rec_type_list) x"
+
 lemma fold_dispatch_wp:
-  "\<lbrakk>proc_ctx_wellformed \<Xi>; upd.proc_env_matches_ptrs \<xi>0 \<Xi>;
-    wa_abs_typing_u (UWA (TPrim (Num U32)) len arr) ''WordArray'' [TPrim (Num U32)] (Boxed ReadOnly ptrl) r w \<sigma>;
-    \<sigma> p = option.Some (UAbstract (UWA (TPrim (Num U32)) len arr));
+  "\<lbrakk>proc_ctx_wellformed \<Xi>; upd.proc_env_matches_ptrs \<xi>0' \<Xi>;
+    wa_abs_typing_u (UWA (TPrim (Num num)) len arr) ''WordArray'' [TPrim (Num num)] (Boxed ReadOnly ptrl) r w \<sigma>;
+    \<sigma> p = option.Some (UAbstract (UWA (TPrim (Num num)) len arr));
     upd.uval_typing \<Xi> \<sigma> acc (foldmap_acc_type ''wordarray_fold_no_break_0'') ra wa;
     upd.uval_typing \<Xi> \<sigma> obsv (foldmap_obsv_type ''wordarray_fold_no_break_0'') ro {};
     wa \<inter> r = {}; wa \<inter> ro = {}; p \<notin> wa;
@@ -855,16 +215,17 @@ lemma fold_dispatch_wp:
     (App f (Var 0)) : (foldmap_funret_type ''wordarray_fold_no_break_0''));
     \<forall>x x' \<sigma> s. val_rel x x' \<longrightarrow>
       update_sem_init.corres wa_abs_typing_u wa_abs_repr (Generated.state_rel wa_abs_repr) 
-        (App f (Var 0)) (do ret <- dispatch_t4' f_num x'; gets (\<lambda>s. ret) od) 
-        \<xi>0 [x] \<Xi> [option.Some (foldmap_funarg_type ''wordarray_fold_no_break_0'')] \<sigma> s\<rbrakk> \<Longrightarrow>
+        (App f (Var 0)) (do ret <- dispatch f_num x'; gets (\<lambda>s. ret) od) 
+        \<xi>0' [x] \<Xi> [option.Some (foldmap_funarg_type ''wordarray_fold_no_break_0'')] \<sigma> s;
+    elem_type (foldmap_funarg_type ''wordarray_fold_no_break_0'') = TPrim (Num num)\<rbrakk> \<Longrightarrow>
     \<lbrace>\<lambda>sa. (a', n') = (a, n) \<and> n < e \<and>
       (\<exists>\<sigma>' res x v. args = t3_C.elem_C_update (\<lambda>_. v) a \<and>
-        \<sigma>' (arr + size_of_num_type U32 * n) = option.Some x \<and> val_rel x v \<and>
-      foldmap_inv upd_wa_foldnb_bod \<xi>0 \<sigma> p frm n f acc obsv (ra \<union> ro) \<sigma>' res sa (t3_C.acc_C args)) \<and>
+        \<sigma>' (arr + size_of_num_type num * n) = option.Some x \<and> val_rel x v \<and>
+      foldmap_inv upd_wa_foldnb_bod \<xi>0' \<sigma> p frm n f acc obsv (ra \<union> ro) \<sigma>' res sa (t3_C.acc_C args)) \<and>
       foldmap_bounds frm to len n e \<and> foldmap_inv_stat obsv (t3_C.obsv_C args)\<rbrace>
-      dispatch_t4' f_num args 
+      dispatch f_num args 
     \<lbrace>\<lambda>ret sb. (\<exists>\<sigma>' res.
-        foldmap_inv upd_wa_foldnb_bod \<xi>0 \<sigma> p frm (n + 1) f acc obsv (ra \<union> ro) \<sigma>' res sb ret) \<and>
+        foldmap_inv upd_wa_foldnb_bod \<xi>0' \<sigma> p frm (n + 1) f acc obsv (ra \<union> ro) \<sigma>' res sb ret) \<and>
       foldmap_inv_stat obsv (t3_C.obsv_C args) \<and> foldmap_bounds frm to len (n + 1) e \<and> 
       foldmap_measure (n + 1) to < foldmap_measure n' to\<rbrace>!"
   apply (subst validNF_def)
@@ -882,7 +243,7 @@ lemma fold_dispatch_wp:
   apply (erule_tac x = \<sigma>' in allE)
   apply (erule_tac x = sa in allE)
   apply (clarsimp simp: corres_def)
-  apply (frule_tac t = "TPrim (Num U32)" in upd_wa_foldnb_bod_preservation[rotated 2]; simp?; clarsimp?)
+  apply (frule_tac t = "TPrim (Num num)" in upd_wa_foldnb_bod_preservation[rotated 2]; simp?; clarsimp?)
   apply (rename_tac r' w')
   apply (subgoal_tac "upd.matches_ptrs \<Xi> \<sigma>' [(mk_urecord [x, res, obsv])]
       [option.Some (foldmap_funarg_type ''wordarray_fold_no_break_0'')] (r' \<union> ro) w'")
@@ -900,12 +261,12 @@ lemma fold_dispatch_wp:
    apply (case_tac "frm < to \<and> frm < len"; clarsimp)
    apply (frule wa_abs_typing_u_elims(5))
    apply (erule_tac x = n in allE; clarsimp)
-   apply (frule_tac p = "arr + 4 * n" in valid_ptr_not_in_frame_same; simp?)
+   apply (frule_tac p = "arr + (size_of_num_type num) * n" in valid_ptr_not_in_frame_same; simp?)
     apply (drule_tac x = "arr + 4 * n" and S' = r in orthD2; simp?)
-    apply (drule_tac t = U32 in  wa_abs_typing_u_elims(2)[where \<tau>s = "[_]", simplified]; simp)
+    apply (drule_tac wa_abs_typing_u_elims(2)[where \<tau>s = "[_]", simplified]; simp)
     apply blast
    apply clarsimp
-   apply (drule_tac t = U32 and arr = arr and len = len and r' = res' 
+   apply (drule_tac t = num and arr = arr and len = len and r' = res' 
       in upd_wa_foldnb_bod_step; simp?; clarsimp?)
     apply (rule conjI)
      apply (drule_tac p = p in readonly_not_in_frame; simp?)
@@ -927,7 +288,7 @@ lemma fold_dispatch_wp:
     apply (frule wa_abs_typing_u_elims(5))
     apply clarsimp
     apply (erule_tac x = i in allE; clarsimp)
-    apply (drule_tac p = "arr + 4 * i" in readonly_not_in_frame; simp?)
+    apply (drule_tac p = "arr + (size_of_num_type num) * i" in readonly_not_in_frame; simp?)
     apply (drule wa_abs_typing_u_elims(2); clarsimp)
     apply blast
    apply (rule conjI)
@@ -958,38 +319,39 @@ lemma fold_dispatch_wp:
   apply (rule upd.matches_ptrs_empty[where \<tau>s = "[]", simplified])
   done
 
-
-lemma upd_C_wordarray_fold_no_break_corres':
-  "\<lbrakk>upd.proc_env_matches_ptrs \<xi>0 \<Xi>; i < length \<gamma>; val_rel (\<gamma> ! i) v'; 
+lemma upd_C_wordarray_fold_no_break_corres_gen:
+  "\<lbrakk>upd.proc_env_matches_ptrs \<xi>0' \<Xi>; i < length \<gamma>; val_rel (\<gamma> ! i) v'; 
     \<Gamma>' ! i = option.Some (prod.fst (prod.snd (\<Xi> ''wordarray_fold_no_break_0'')));
-    \<gamma> ! i = URecord fs; f = prod.fst (fs ! 3); obsv = prod.fst (fs ! 5);
-    upd.uval_typing \<Xi> \<sigma> obsv (foldmap_obsv_type ''wordarray_fold_no_break_0'') ro {};
+    D \<in> k \<or> S \<in> k; K' \<turnstile> (foldmap_obsv_type ''wordarray_fold_no_break_0'') :\<kappa> k;
+    \<gamma> ! i = URecord fs; f = prod.fst (fs ! 3);  
     (\<Xi>, [], [option.Some (foldmap_funarg_type ''wordarray_fold_no_break_0'')] \<turnstile> 
     (App (uvalfun_to_exprfun f) (Var 0)) : (foldmap_funret_type ''wordarray_fold_no_break_0''));
     \<forall>x x' \<sigma> s. val_rel x x' \<longrightarrow> update_sem_init.corres wa_abs_typing_u wa_abs_repr (Generated.state_rel wa_abs_repr) 
       (App (uvalfun_to_exprfun f) (Var 0)) (do ret <- dispatch_t4' (t5_C.f_C v') x'; gets (\<lambda>s. ret) od) 
-      \<xi>0 [x] \<Xi> [option.Some (foldmap_funarg_type ''wordarray_fold_no_break_0'')] \<sigma> s\<rbrakk>
+      \<xi>0' [x] \<Xi> [option.Some (foldmap_funarg_type ''wordarray_fold_no_break_0'')] \<sigma> s;
+    \<xi>1' ''wordarray_fold_no_break_0'' = upd_wa_foldnb \<Xi> \<xi>0' (foldmap_funarg_type ''wordarray_fold_no_break_0'');
+    elem_type (foldmap_funarg_type ''wordarray_fold_no_break_0'') = TPrim (Num num)\<rbrakk>
     \<Longrightarrow> update_sem_init.corres wa_abs_typing_u wa_abs_repr (Generated.state_rel wa_abs_repr)
          (App (AFun ''wordarray_fold_no_break_0'' []) (Var i)) (do x <- main_pp_inferred.wordarray_fold_no_break_0' v';
 gets (\<lambda>s. x)
                                                                 od)
-         \<xi>1 \<gamma> \<Xi>  \<Gamma>' \<sigma> s"
+         \<xi>1' \<gamma> \<Xi>  \<Gamma>' \<sigma> s"
   apply (rule absfun_corres; simp)
   apply (clarsimp simp: abs_fun_rel_def'; rename_tac r w)
   apply (thin_tac "\<Gamma>' ! i = _")
-  apply (subst \<xi>1.simps)
   apply (subst (asm) val_rel_simp; clarsimp)
   apply (subst (asm) val_rel_ptr_def; clarsimp)
   apply (subst (asm) val_rel_fun_tag)
   apply (subst (asm) val_rel_word)
   apply (subst (asm) val_rel_word)
   apply (clarsimp simp: upd_wa_foldnb_def wordarray_fold_no_break_0'_def)
-  apply (rename_tac pwa_rep frm_rep to_rep f_rep acc a_rep o_rep wa_rep)
+  apply (rename_tac pwa_rep frm_rep to_rep f_rep acc a_rep obsv o_rep wa_rep)
   apply (erule upd.u_t_recE; clarsimp)
   apply (clarsimp simp: \<Xi>_wordarray_fold_no_break_0 wordarray_fold_no_break_0_type_def abbreviated_type_defs)
   apply (erule upd.u_t_r_consE; clarsimp)
   apply (erule upd.u_t_p_absE; clarsimp)
   apply (frule wa_abs_typing_u_elims(1); clarsimp)
+  apply (rename_tac r len arr)
   apply (erule upd.u_t_r_consE; simp)
   apply (erule upd.u_t_r_consE; simp)
   apply (erule conjE)+
@@ -1003,8 +365,8 @@ gets (\<lambda>s. x)
   apply (frule upd.tfun_no_pointers(1))
   apply (frule upd.tfun_no_pointers(2))
   apply clarsimp
-  apply (rename_tac acc ra wa ro' wo)
-  apply (drule_tac x = obsv in upd.uval_typing_unique_ptrs(1); simp?)
+  apply (rename_tac acc ra wa obsv ro wo)
+  apply (drule upd.discardable_or_shareable_not_writeable; simp?)
   apply clarsimp
   apply (subst unknown_bind_ignore)+
   apply (clarsimp simp: join_guards)
@@ -1012,7 +374,7 @@ gets (\<lambda>s. x)
       apply (clarsimp simp: unknown_bind_ignore split: prod.split)
       apply (rename_tac var e)
       apply (rule_tac M = "\<lambda>((_, i), _). foldmap_measure i (t5_C.to_C v')" and 
-      I = "\<lambda>(a, b) s. (\<exists>\<sigma>' res. foldmap_inv upd_wa_foldnb_bod \<xi>0 \<sigma> (ptr_val (t5_C.arr_C v'))
+      I = "\<lambda>(a, b) s. (\<exists>\<sigma>' res. foldmap_inv upd_wa_foldnb_bod \<xi>0' \<sigma> (ptr_val (t5_C.arr_C v'))
           (t5_C.frm_C v') b (uvalfun_to_exprfun f) acc obsv (ra \<union> ro) \<sigma>' res s (t3_C.acc_C a)) \<and>
           foldmap_inv_stat obsv (t3_C.obsv_C a) \<and>
           foldmap_bounds (t5_C.frm_C v') (t5_C.to_C v') len b e" in whileLoop_add_invI; simp?)
@@ -1031,8 +393,8 @@ gets (\<lambda>s. x)
        apply (drule_tac acc = acc and obsv = obsv and rb = ra and wb = wa and rc = ro
           in upd_wa_foldnb_bod_preservation; simp?; clarsimp?)
        apply (frule_tac p = "ptr_val (t5_C.arr_C v')" in valid_ptr_not_in_frame_same; simp?)
-       apply (drule_tac p = "arr + 4 * j" in valid_ptr_not_in_frame_same; simp?)
-        apply (drule_tac x = "arr + 4 * j" and S = wa and S' = r in orthD2; simp?)
+       apply (drule_tac p = "arr + (size_of_num_type num) * j" in valid_ptr_not_in_frame_same; simp?)
+        apply (drule_tac x = "arr + (size_of_num_type num) * j" and S = wa and S' = r in orthD2; simp?)
         apply (drule wa_abs_typing_u_elims(2); clarsimp)
         apply blast
        apply (thin_tac "_ \<in> state_rel")
@@ -1043,15 +405,15 @@ gets (\<lambda>s. x)
         apply clarsimp
         apply (clarsimp simp: state_rel_def heap_rel_def heap_rel_ptr_w32_meta heap_rel_ptr_meta)
         apply (rotate_tac -1)
-        apply (drule_tac p = "Ptr(arr + 4 * j)" in all_heap_rel_ptrD; simp?)
+        apply (drule_tac p = "Ptr(arr + (size_of_num_type num) * j)" in all_heap_rel_ptrD; simp?)
          apply (clarsimp simp: type_rel_simp)
-        apply (rule_tac x = "heap_w32 s (PTR(32 word) (arr + 4 * j))" in exI)
+        apply (rule_tac x = "heap_w32 s (PTR(32 word) (arr + (size_of_num_type num) * j))" in exI)
         apply (drule_tac p = "t5_C.arr_C v'" in all_heap_rel_ptrD; simp?)
          apply (clarsimp simp: type_rel_simp wa_abs_repr_def)
         apply (clarsimp simp: val_rel_WordArray_u32_C_def ptr_add_def heap_simp mult.commute)
        apply (clarsimp simp: state_rel_def heap_rel_def heap_rel_ptr_w32_meta heap_rel_ptr_meta)
        apply (rotate_tac -1)
-       apply (drule_tac p = "Ptr(arr + 4 * j)" in all_heap_rel_ptrD; simp?)
+       apply (drule_tac p = "Ptr(arr + (size_of_num_type num) * j)" in all_heap_rel_ptrD; simp?)
         apply (clarsimp simp: type_rel_simp)
        apply (drule_tac p = "t5_C.arr_C v'" in all_heap_rel_ptrD; simp?)
         apply (clarsimp simp: type_rel_simp wa_abs_repr_def)
@@ -1132,9 +494,9 @@ lemma \<Xi>_wordarray_map_no_break_0:
   by (clarsimp simp: \<Xi>_def)
 
 lemma map_dispatch_wp:
-  "\<lbrakk>proc_ctx_wellformed \<Xi>; upd.proc_env_matches_ptrs \<xi>0 \<Xi>;
-    wa_abs_typing_u (UWA (TPrim (Num U32)) len arr) ''WordArray'' [TPrim (Num U32)] (Boxed Writable ptrl) r w \<sigma>;
-    \<sigma> p = option.Some (UAbstract (UWA (TPrim (Num U32)) len arr));
+  "\<lbrakk>proc_ctx_wellformed \<Xi>; upd.proc_env_matches_ptrs \<xi>0' \<Xi>;
+    wa_abs_typing_u (UWA (TPrim (Num num)) len arr) ''WordArray'' [TPrim (Num num)] (Boxed Writable ptrl) r w \<sigma>;
+    \<sigma> p = option.Some (UAbstract (UWA (TPrim (Num num)) len arr));
     upd.uval_typing \<Xi> \<sigma> acc (foldmap_acc_type ''wordarray_map_no_break_0'') ra wa;
     upd.uval_typing \<Xi> \<sigma> obsv (foldmap_obsv_type ''wordarray_map_no_break_0'') ro {}; wa \<inter> r = {}; p \<notin> w;
     p \<notin> r; w \<inter> wa = {}; w \<inter> (ra \<union> ro) = {}; wa \<inter> ro = {}; p \<notin> wa; p \<notin> ra; p \<notin> ro; p = ptr_val p';
@@ -1142,16 +504,17 @@ lemma map_dispatch_wp:
     (App f (Var 0)) : (foldmap_funret_type ''wordarray_map_no_break_0''));
     \<forall>x x' \<sigma> s. val_rel x x' \<longrightarrow>
       update_sem_init.corres wa_abs_typing_u wa_abs_repr (Generated.state_rel wa_abs_repr) 
-        (App f (Var 0)) (do ret <- dispatch_t8' f_num x'; gets (\<lambda>s. ret) od) 
-        \<xi>0 [x] \<Xi> [option.Some (foldmap_funarg_type ''wordarray_map_no_break_0'')] \<sigma> s\<rbrakk> \<Longrightarrow>
+        (App f (Var 0)) (do ret <- dispatch f_num x'; gets (\<lambda>s. ret) od) 
+        \<xi>0' [x] \<Xi> [option.Some (foldmap_funarg_type ''wordarray_map_no_break_0'')] \<sigma> s;
+     elem_type (foldmap_funarg_type ''wordarray_map_no_break_0'') = TPrim (Num num)\<rbrakk> \<Longrightarrow>
     \<lbrace>\<lambda>sa. (a', n') = (a, n) \<and> n < e \<and>
       (\<exists>\<sigma>' res x v. args = t6_C.elem_C_update (\<lambda>_. v) a \<and>
         \<sigma>' (arr + size_of_num_type U32 * n) = option.Some x \<and> val_rel x v \<and>
-      foldmap_inv upd_wa_mapAccumnb_bod \<xi>0 \<sigma> p frm n f acc obsv (ra \<union> ro) \<sigma>' res sa (t10_C p' (t6_C.acc_C args))) \<and>
+      foldmap_inv upd_wa_mapAccumnb_bod \<xi>0' \<sigma> p frm n f acc obsv (ra \<union> ro) \<sigma>' res sa (t10_C p' (t6_C.acc_C args))) \<and>
       foldmap_bounds frm to len n e \<and> foldmap_inv_stat obsv (t6_C.obsv_C args)\<rbrace>
-      dispatch_t8' f_num args 
+      dispatch f_num args 
      \<lbrace>\<lambda>ret sb. (\<exists>\<sigma>' res. 
-        foldmap_inv upd_wa_mapAccumnb_bod \<xi>0 \<sigma> p frm (n + 1) f acc obsv (ra \<union> ro) \<sigma>' res 
+        foldmap_inv upd_wa_mapAccumnb_bod \<xi>0' \<sigma> p frm (n + 1) f acc obsv (ra \<union> ro) \<sigma>' res 
           (heap_w32_update (\<lambda>x a. if a = values_C (heap_WordArray_u32_C sb p') +\<^sub>p uint n 
             then t7_C.p1_C ret else x a) sb) (t10_C p' (t7_C.p2_C ret))) \<and>
         foldmap_inv_stat obsv (t6_C.obsv_C args) \<and>
@@ -1178,7 +541,7 @@ lemma map_dispatch_wp:
   apply (erule_tac x = \<sigma>' in allE)
   apply (erule_tac x = sa in allE)
   apply (clarsimp simp: corres_def)
-  apply (frule_tac t = "TPrim (Num U32)" in upd_wa_mapAccumnb_bod_preservation; simp?; clarsimp?)
+  apply (frule_tac t = "TPrim (Num num)" in upd_wa_mapAccumnb_bod_preservation; simp?; clarsimp?)
     apply (subst Int_Un_distrib2; clarsimp)
     apply (subst (asm) Int_Un_distrib; clarsimp)
    apply (subst (asm) Int_Un_distrib; clarsimp)
@@ -1219,7 +582,7 @@ lemma map_dispatch_wp:
    apply (clarsimp simp: foldmap_bounds_def)
    apply (case_tac "frm < to \<and> frm < len"; clarsimp)
    apply (thin_tac "wa_abs_typing_u _ _ _ _ _ _ _")
-   apply (drule_tac t = U32 and arr = arr and len = len and v' = x' and r' = racc'
+   apply (drule_tac t = num and arr = arr and len = len and v' = x' and r' = racc'
       in upd_wa_mapAccumnb_bod_step; simp?; clarsimp?)
       apply (drule wa_abs_typing_u_elims(6); simp?)
      apply (subst Int_Un_distrib2)+
@@ -1246,8 +609,8 @@ lemma map_dispatch_wp:
    apply (thin_tac "_ \<in> state_rel")
    apply (clarsimp simp: state_rel_def heap_rel_def heap_rel_ptr_meta heap_rel_ptr_w32_meta)
    apply (frule_tac p = p and \<sigma> = \<sigma>' in valid_ptr_not_in_frame_same; simp?)
-   apply (drule_tac p = "arr + 4 * n" and \<sigma> = \<sigma>' in valid_ptr_not_in_frame_same; simp?)
-    apply (drule_tac x = "arr + 4 * n" and S' = wc in orthD1; simp?)
+   apply (drule_tac p = "arr + (size_of_num_type num) * n" and \<sigma> = \<sigma>' in valid_ptr_not_in_frame_same; simp?)
+    apply (drule_tac x = "arr + (size_of_num_type num) * n" and S' = wc in orthD1; simp?)
     apply (drule wa_abs_typing_u_elims(3); clarsimp)
     apply (rule_tac x = n in exI; clarsimp)
    apply (frule_tac p = p' in all_heap_rel_ptrD; simp?)
@@ -1256,7 +619,7 @@ lemma map_dispatch_wp:
      apply (clarsimp simp: val_rel_simp heap_simp)
     apply (clarsimp simp: type_rel_simp val_rel_simp)
    apply (rule conjI)
-    apply (rule_tac x = "\<sigma>''(arr + 4 * n \<mapsto> x')" in exI)
+    apply (rule_tac x = "\<sigma>''(arr + (size_of_num_type num) * n \<mapsto> x')" in exI)
     apply (rule_tac x = "mk_urecord [UPtr (ptr_val p') (RCon ''WordArray'' [RPrim (Num U32)]), racc']" in exI)
     apply clarsimp
     apply (rule conjI)
@@ -1306,25 +669,27 @@ lemma map_dispatch_wp:
   apply (rule upd.matches_ptrs_empty[where \<tau>s = "[]", simplified])
   done
 
-lemma upd_C_wordarray_map_no_break_corres':
-  "\<lbrakk>upd.proc_env_matches_ptrs \<xi>0 \<Xi>; i < length \<gamma>; val_rel (\<gamma> ! i) v';
+lemma upd_C_wordarray_map_no_break_corres_gen:
+  "\<lbrakk>upd.proc_env_matches_ptrs \<xi>0' \<Xi>; i < length \<gamma>; val_rel (\<gamma> ! i) v';
     \<Gamma>' ! i = option.Some (prod.fst (prod.snd (\<Xi> ''wordarray_map_no_break_0'')));
-    \<gamma> ! i = URecord fs; f = prod.fst (fs ! 3); obsv = prod.fst (fs ! 5);
-    upd.uval_typing \<Xi> \<sigma> obsv (foldmap_obsv_type ''wordarray_map_no_break_0'') ro {};
+     D \<in> k \<or> S \<in> k; K' \<turnstile> (foldmap_obsv_type ''wordarray_map_no_break_0'') :\<kappa> k;
+    \<gamma> ! i = URecord fs; f = prod.fst (fs ! 3);
     (\<Xi>, [], [option.Some (foldmap_funarg_type ''wordarray_map_no_break_0'')] \<turnstile> 
     (App (uvalfun_to_exprfun f) (Var 0)) : (foldmap_funret_type ''wordarray_map_no_break_0''));
     \<forall>x x' \<sigma> s. val_rel x x' \<longrightarrow> update_sem_init.corres wa_abs_typing_u wa_abs_repr (Generated.state_rel wa_abs_repr) 
       (App (uvalfun_to_exprfun f) (Var 0)) (do ret <- dispatch_t8' (t9_C.f_C v') x'; gets (\<lambda>s. ret) od) 
-      \<xi>0 [x] \<Xi> [option.Some (foldmap_funarg_type ''wordarray_map_no_break_0'')] \<sigma> s\<rbrakk>
+      \<xi>0' [x] \<Xi> [option.Some (foldmap_funarg_type ''wordarray_map_no_break_0'')] \<sigma> s;
+    \<xi>1' ''wordarray_map_no_break_0'' = upd_wa_mapAccumnb \<Xi> \<xi>0' 
+      (foldmap_funarg_type ''wordarray_map_no_break_0'') (foldmap_funret_type ''wordarray_map_no_break_0'');
+    elem_type (foldmap_funarg_type ''wordarray_map_no_break_0'') = TPrim (Num num)\<rbrakk>
     \<Longrightarrow> update_sem_init.corres wa_abs_typing_u wa_abs_repr (Generated.state_rel wa_abs_repr)
          (App (AFun ''wordarray_map_no_break_0'' []) (Var i)) (do x <- main_pp_inferred.wordarray_map_no_break_0' v';
 gets (\<lambda>s. x)
                                                                 od)
-         \<xi>1 \<gamma> \<Xi>  \<Gamma>' \<sigma> s"
+         \<xi>1' \<gamma> \<Xi>  \<Gamma>' \<sigma> s"
   apply (rule absfun_corres; simp)
   apply (clarsimp simp: abs_fun_rel_def'; rename_tac r w)
   apply (thin_tac "\<Gamma>' ! i = _")
-  apply (subst \<xi>1.simps)
   apply (subst (asm) val_rel_simp; clarsimp)
   apply (subst (asm) val_rel_ptr_def; clarsimp)
   apply (subst (asm) val_rel_fun_tag)
@@ -1339,6 +704,7 @@ gets (\<lambda>s. x)
   apply (erule upd.u_t_p_absE; clarsimp)
   apply (rename_tac w)
   apply (frule wa_abs_typing_u_elims(1); clarsimp)
+  apply (rename_tac len arr)
   apply (erule upd.u_t_r_consE; simp)
   apply (erule upd.u_t_r_consE; simp)
   apply (erule conjE)+
@@ -1352,15 +718,15 @@ gets (\<lambda>s. x)
   apply (frule upd.tfun_no_pointers(1))
   apply (frule upd.tfun_no_pointers(2))
   apply clarsimp
-  apply (rename_tac acc ra wa ro' wo)
-  apply (drule_tac x = obsv in upd.uval_typing_unique_ptrs(1); simp?)
+  apply (rename_tac acc ra wa obsv ro wo)
+  apply (drule_tac v = obsv in upd.discardable_or_shareable_not_writeable(1); simp?)
   apply (subst unknown_bind_ignore)+
   apply (clarsimp simp: join_guards) 
   apply wp
       apply (clarsimp simp: unknown_bind_ignore split: prod.split)
        apply (rename_tac var e)
        apply (rule_tac M = "\<lambda>((_, i), _). foldmap_measure i (t9_C.to_C v')" and 
-      I = "\<lambda>(a, b) s. (\<exists>\<sigma>' res. foldmap_inv upd_wa_mapAccumnb_bod \<xi>0 \<sigma> (ptr_val (t9_C.arr_C v'))
+      I = "\<lambda>(a, b) s. (\<exists>\<sigma>' res. foldmap_inv upd_wa_mapAccumnb_bod \<xi>0' \<sigma> (ptr_val (t9_C.arr_C v'))
           (t9_C.frm_C v') b (uvalfun_to_exprfun f) acc obsv (ra \<union> ro) \<sigma>' res s (t10_C (t9_C.arr_C v') (t6_C.acc_C a))) \<and>
           foldmap_inv_stat obsv (t6_C.obsv_C a) \<and>
           foldmap_bounds (t9_C.frm_C v') (t9_C.to_C v') len b e" in whileLoop_add_invI; simp?)
@@ -1397,14 +763,14 @@ gets (\<lambda>s. x)
         apply (frule_tac p = "t9_C.arr_C v'" in all_heap_rel_ptrD; simp?)
          apply (clarsimp simp: type_rel_simp wa_abs_repr_def)
         apply (rotate_tac -2)
-         apply (frule_tac p = "Ptr(arr + 4 * j)" in all_heap_rel_ptrD; simp?)
+         apply (frule_tac p = "Ptr(arr + (size_of_num_type num) * j)" in all_heap_rel_ptrD; simp?)
          apply (clarsimp simp: type_rel_simp)
         apply (rule conjI)
          apply (rule_tac x = \<sigma>' in exI)
          apply (rule_tac x = "mk_urecord [UPtr (ptr_val (t9_C.arr_C v'))
-          (RCon ''WordArray'' [RPrim (Num U32)]), racc]" in exI)
+          (RCon ''WordArray'' [RPrim (Num num)]), racc]" in exI)
          apply (rule_tac x = "UPrim x" in exI)
-         apply (rule_tac x = "heap_w32 s (PTR(32 word) (arr + 4 * j))" in exI)
+         apply (rule_tac x = "heap_w32 s (PTR(32 word) (arr + (size_of_num_type num) * j))" in exI)
          apply (clarsimp simp: val_rel_WordArray_u32_C_def ptr_add_def heap_simp mult.commute)
         apply (clarsimp simp: val_rel_WordArray_u32_C_def ptr_add_def is_valid_simp heap_simp mult.commute)
        apply (rule conjI)
@@ -1461,7 +827,7 @@ gets (\<lambda>s. x)
    apply (rule conjI)
     apply (rule_tac x = \<sigma> in exI)
     apply (rule_tac x = "mk_urecord [UPtr (ptr_val (t9_C.arr_C v'))
-      (RCon ''WordArray'' [RPrim (Num U32)]), acc]" in exI)
+      (RCon ''WordArray'' [RPrim (Num num)]), acc]" in exI)
     apply (subst upd_wa_mapAccumnb_bod.simps; clarsimp)
     apply (rule conjI)
      apply (drule wa_abs_typing_u_elims(5); clarsimp)
@@ -1478,7 +844,7 @@ gets (\<lambda>s. x)
   apply (rule conjI)
    apply (rule_tac x = \<sigma> in exI)
    apply (rule_tac x = "mk_urecord [UPtr (ptr_val (t9_C.arr_C v'))
-      (RCon ''WordArray'' [RPrim (Num U32)]), acc]" in exI)
+      (RCon ''WordArray'' [RPrim (Num num)]), acc]" in exI)
    apply (subst upd_wa_mapAccumnb_bod.simps; clarsimp)
    apply (rule conjI)
     apply (drule wa_abs_typing_u_elims(5); clarsimp)
@@ -1492,84 +858,6 @@ gets (\<lambda>s. x)
   apply (subst min_def)
   apply (clarsimp simp: not_le)
   done
-
-lemma 
-" \<And>v' i \<gamma> \<Gamma> \<sigma> s.
-        \<lbrakk>t9_C.f_C v' = FUN_ENUM_dec; i < length \<gamma>; val_rel (\<gamma> ! i) v';
-         \<Gamma> ! i =
-         option.Some
-          (prod.fst
-            (prod.snd
-              (assoc_lookup
-                [(''wordarray_get_0'', wordarray_get_0_type), (''wordarray_length_0'', wordarray_length_0_type),
-                 (''wordarray_put2_0'', wordarray_put2_0_type), (''wordarray_fold_no_break_0'', wordarray_fold_no_break_0_type),
-                 (''wordarray_map_no_break_0'', wordarray_map_no_break_0_type),
-                 (''wordarray_get_u32'', Generated_TypeProof.wordarray_get_u32_type),
-                 (''wordarray_length_u32'', Generated_TypeProof.wordarray_length_u32_type),
-                 (''wordarray_put2_u32'', Generated_TypeProof.wordarray_put2_u32_type), (''dec'', Generated_TypeProof.dec_type),
-                 (''dec_arr'', Generated_TypeProof.dec_arr_type), (''inc'', Generated_TypeProof.inc_type),
-                 (''inc_arr'', Generated_TypeProof.inc_arr_type), (''mul'', Generated_TypeProof.mul_type),
-                 (''mul_arr'', Generated_TypeProof.mul_arr_type), (''sum'', Generated_TypeProof.sum_type),
-                 (''sum_arr'', Generated_TypeProof.sum_arr_type)]
-                ([], TUnit, TUnit) ''wordarray_map_no_break_0'')))\<rbrakk>
-        \<Longrightarrow> update_sem_init.corres wa_abs_typing_u wa_abs_repr (Generated.state_rel wa_abs_repr)
-             (App (AFun ''wordarray_map_no_break_0'' []) (Var i)) (do x <- wordarray_map_no_break_0' v';
-     gets (\<lambda>s. x)
-  od)
-             \<xi>1 \<gamma>
-             (assoc_lookup
-               [(''wordarray_get_0'', wordarray_get_0_type), (''wordarray_length_0'', wordarray_length_0_type),
-                (''wordarray_put2_0'', wordarray_put2_0_type), (''wordarray_fold_no_break_0'', wordarray_fold_no_break_0_type),
-                (''wordarray_map_no_break_0'', wordarray_map_no_break_0_type),
-                (''wordarray_get_u32'', Generated_TypeProof.wordarray_get_u32_type),
-                (''wordarray_length_u32'', Generated_TypeProof.wordarray_length_u32_type),
-                (''wordarray_put2_u32'', Generated_TypeProof.wordarray_put2_u32_type), (''dec'', Generated_TypeProof.dec_type),
-                (''dec_arr'', Generated_TypeProof.dec_arr_type), (''inc'', Generated_TypeProof.inc_type),
-                (''inc_arr'', Generated_TypeProof.inc_arr_type), (''mul'', Generated_TypeProof.mul_type),
-                (''mul_arr'', Generated_TypeProof.mul_arr_type), (''sum'', Generated_TypeProof.sum_type),
-                (''sum_arr'', Generated_TypeProof.sum_arr_type)]
-               ([], TUnit, TUnit))
-             \<Gamma> \<sigma> s"
-  apply (subst (asm) \<Xi>_def[symmetric])
-  apply (subst \<Xi>_def[symmetric])
-  apply (subst (asm) val_rel_simp; clarsimp)
-  apply (rename_tac wp wpr frm frmr to tor f fr acc accr obsv obsvr)
-  apply (drule_tac v' = v' and \<sigma> = \<sigma> and s = s and ro = "{}" in upd_C_wordarray_map_no_break_corres'[rotated 1]; simp?)
-       apply (clarsimp simp: val_rel_simp)
-      apply (clarsimp simp: \<Xi>_wordarray_map_no_break_0 wordarray_map_no_break_0_type_def abbreviated_type_defs val_rel_simp)
-      apply (rule upd.u_t_unit)
-     apply (rule typing_app[of _ _ 
-        "[option.Some (foldmap_funarg_type ''wordarray_map_no_break_0'')]"
-        "[option.Some (foldmap_funarg_type ''wordarray_map_no_break_0'')]"
-        _ _  "(foldmap_funarg_type ''wordarray_map_no_break_0'')"]; simp?)
-       apply (rule split_cons[where xs = "[]" and ys = "[]" and zs = "[]", simplified])
-        apply (rule_tac k = "kinding_fn [] (foldmap_funarg_type ''wordarray_map_no_break_0'')" in share; simp?)
-         apply (rule kindingI; simp?)
-         apply (clarsimp simp: \<Xi>_wordarray_map_no_break_0 wordarray_map_no_break_0_type_def abbreviated_type_defs)
-        apply (clarsimp simp: \<Xi>_wordarray_map_no_break_0 wordarray_map_no_break_0_type_def abbreviated_type_defs)
-       apply (rule split_empty)
-      apply (clarsimp simp: \<Xi>_def cogent_function_val_rel val_rel_fun_tag untyped_func_enum_defs wordarray_map_no_break_0_type_def abbreviated_type_defs)
-      apply (rule typing_fun; simp?; clarsimp?)
-       apply (subst abbreviated_type_defs[symmetric])+
-       apply (subst wordarray_map_no_break_0_type_def[symmetric])+
-       apply (subst \<Xi>_def[symmetric])
-       apply (cut_tac dec_typecorrect')
-       apply (clarsimp simp: dec_type_def)
-      apply (clarsimp simp: empty_def weakening_Cons[where xs = "[]" and ys = "[]", simplified])
-      apply (rule conjI)
-       apply (rule_tac k = "{D, S, E}" in drop; simp?)
-       apply (rule kindingI; clarsimp)
-      apply (rule weakening_nil)
-     apply (rule typing_var; clarsimp)
-     apply (clarsimp simp: empty_def weakening_Cons[where xs = "[]" and ys = "[]", simplified])
-     apply (rule conjI)
-      apply (rule keep; clarsimp simp: \<Xi>_wordarray_map_no_break_0 wordarray_map_no_break_0_type_def abbreviated_type_defs)
-     apply (rule weakening_nil)
-  
-
-
-  oops
-  value "((ucast (1 :: 64 word)) :: 32 word)"
 
 end (* of context *)
 end
