cogent/examples/wa_connect/Sum_Corres.thy
@@ -1,0 +1,583 @@
+theory Sum_Corres
+imports WordArray_SVCorres WordArray_UpdCCorres WordArray_CorresProof_Asm
+
+begin
+
+text
+  "This is an example of proving that @{term main_pp_inferred.sum_arr'} refines
+  @{term Generated_Shallow_Desugar.sum_arr}. We can show this if we can prove that
+  @{thm Generated_cogent_shallow.corres_shallow_C_sum_arr} is true without
+  assuming that the abstract functions refine their corresponding shallow embeddings.
+
+  @{term Generated_Shallow_Desugar.sum_arr} depends on the abstract functions defined for word
+  arrays. So if we want to prove that our compilation is correct for 
+  @{term Generated_Shallow_Desugar.sum_arr}, we need to prove that the "
+
+context WordArray begin
+text 
+  "The two word array functions that we need to manually verify are @{term wordarray_length} and
+   @{term wordarray_fold_no_break}"
+lemma sum_corres:
+  "val_rel a a' \<Longrightarrow>
+  corres state_rel Generated_TypeProof.sum (local.sum' a') \<xi>' [a] \<Xi>
+  [option.Some (prod.fst (prod.snd Generated_TypeProof.sum_type))] \<sigma> s"
+  apply (unfold sum_def sum'_def sum_type_def abbreviated_type_defs val_rel_simp)
+  apply (elim exE conjE)
+  apply (subst unknown_bind_ignore)
+  apply (subst snd_conv)
+  apply (subst fst_conv)
+  apply (monad_eq simp: corres_def)
+  apply (intro exI conjI; (simp add: val_rel_simp)?)
+  apply (rule u_sem_take_ub)
+   apply (rule u_sem_var[of _ "[_]" _ 0, simplified])
+  apply clarsimp
+  apply (rule u_sem_take_ub; simp?)
+   apply (rule u_sem_var[of _ "[_, _, _]" _ "Suc 0", simplified])
+  apply clarsimp
+  apply (rule u_sem_take_ub; simp?)
+   apply (rule u_sem_var[of _ "[_, _, _, _, _]" _ "Suc 0", simplified])
+  apply clarsimp
+  apply (rename_tac b ba bb r x)
+  apply (cut_tac 
+      \<gamma> = "[UUnit,
+            URecord [(UPrim (LU32 (t3_C.elem_C a')), b), (UPrim (LU32 (t3_C.acc_C a')), ba), (UUnit, bb)],
+            UPrim (LU32 (t3_C.acc_C a')),
+            URecord [(UPrim (LU32 (t3_C.elem_C a')), b), (UPrim (LU32 (t3_C.acc_C a')), ba), (UUnit, bb)],
+            UPrim (LU32 (t3_C.elem_C a')),
+            URecord [(UPrim (LU32 (t3_C.elem_C a')), b), (UPrim (LU32 (t3_C.acc_C a')), ba), (UUnit, bb)],
+            URecord [(UPrim (LU32 (t3_C.elem_C a')), b), (UPrim (LU32 (t3_C.acc_C a')), ba), (UUnit, bb)]]"
+      in u_sem_prim[of \<xi>' _ \<sigma> "[Var 4, Var 2]" \<sigma> 
+        "[UPrim (LU32 (t3_C.elem_C a')), UPrim (LU32 (t3_C.acc_C a'))]" "Plus U32"])
+   apply (rule u_sem_all_cons[of _ _ _ _ \<sigma>])
+    apply (rule u_sem_var[of _ "[_, _, _, _, _, _, _]" _ "4", simplified])
+   apply (rule u_sem_all_cons[of _ _ _ _ \<sigma>])
+    apply (rule u_sem_var[of _ "[_, _, _, _, _, _, _]" _ "2", simplified])
+   apply (rule u_sem_all_empty)
+  apply (clarsimp simp: eval_prim_u_def)
+  done
+
+lemma sum_arr_corres:
+  "\<lbrakk>\<And>i \<gamma> v' \<Gamma>' \<sigma> st.
+    \<lbrakk>i < length \<gamma>; val_rel (\<gamma> ! i) v';
+     \<Gamma>' ! i = option.Some (prod.fst (prod.snd (\<Xi> ''wordarray_length_0'')))\<rbrakk>
+    \<Longrightarrow> corres state_rel (App (AFun ''wordarray_length_0'' []) (Var i))
+      (do x <- wordarray_length_0' v'; gets (\<lambda>s. x) od) \<xi>' \<gamma> \<Xi>  \<Gamma>' \<sigma> st;
+    \<And>v' i \<gamma> \<Gamma> \<sigma> s.
+    \<lbrakk>t5_C.f_C v' = FUN_ENUM_sum; i < length \<gamma>; val_rel (\<gamma> ! i) v';
+     \<Gamma> ! i = option.Some (prod.fst (prod.snd (\<Xi> ''wordarray_fold_no_break_0'')))\<rbrakk>
+    \<Longrightarrow> corres state_rel (App (AFun ''wordarray_fold_no_break_0'' []) (Var i))
+      (do x <- wordarray_fold_no_break_0' v'; gets (\<lambda>s. x) od) \<xi>' \<gamma> \<Xi> \<Gamma> \<sigma> s;
+    val_rel a a'\<rbrakk>
+    \<Longrightarrow> corres state_rel Generated_TypeProof.sum_arr (sum_arr' a') \<xi>' [a] \<Xi>
+     [option.Some (prod.fst (prod.snd Generated_TypeProof.sum_arr_type))] \<sigma> s"
+  apply (unfold sum_arr_def sum_arr'_def sum_arr_type_def abbreviated_type_defs val_rel_simp cogent_function_val_rel)
+  apply (elim exE conjE)
+  apply (subst unknown_bind_ignore)
+  apply (subst snd_conv)
+  apply (subst fst_conv)
+  apply (monad_eq simp: corres_def)
+  apply (drule_tac x = 0 in meta_spec)
+  apply (drule_tac x = "[a]" in meta_spec)
+  apply (drule_tac x = a' in meta_spec)
+  apply clarsimp
+  apply (drule_tac x = "[option.Some (prod.fst (prod.snd (\<Xi> ''wordarray_length_0'')))]" in meta_spec)
+  apply (drule_tac x = \<sigma> in meta_spec)
+  apply (drule_tac x = s in meta_spec)
+  apply clarsimp
+  apply (rename_tac repr r w)
+  apply (erule impE)
+   apply (rule_tac x = r in exI)
+   apply (rule_tac x = w in exI)
+   apply (clarsimp simp: \<Xi>_def wordarray_length_0_type_def abbreviated_type_defs)
+  apply clarsimp
+  apply (intro exI conjI; (simp add: val_rel_simp)?)
+   apply (rule allI)+
+   apply (rename_tac r' s')
+   apply (erule_tac x = r' in allE)
+   apply (erule_tac x = s' in allE)
+   apply (rule impI)
+   apply (erule impE, assumption)
+   apply (drule_tac x = "t5_C a' 0 r' FUN_ENUM_sum 0 (unit_t_C 0)" in meta_spec)
+   apply (drule_tac x = 0 in meta_spec)
+   apply clarsimp
+   apply (drule_tac 
+      x = "[mk_urecord [UPtr (ptr_val a') repr, 
+            UPrim (LU32 0), UPrim (LU32 r'),  
+            UFunction Generated_TypeProof.sum [], 
+            UPrim (LU32 0), 
+            UUnit]]" in meta_spec)
+   apply clarsimp
+   apply (drule_tac x = "[option.Some (prod.fst (prod.snd (\<Xi> ''wordarray_fold_no_break_0'')))]" in meta_spec)
+   apply (rename_tac \<sigma>')
+   apply (drule_tac x = \<sigma>' in meta_spec)
+   apply (drule_tac x = s' in meta_spec)
+   apply clarsimp
+   apply (elim u_sem_appE u_sem_afunE u_sem_funE u_sem_varE; simp?)
+   apply (erule upd.matches_ptrs_consE; clarsimp)
+   apply (rename_tac ra wa rb wb)
+   apply (drule upd.proc_env_matches_ptrs_abstract[where \<tau>s = "[]", simplified]; simp?,
+      (simp add: \<Xi>_def wordarray_length_0_type_def abbreviated_type_defs)?)
+   apply (clarsimp simp: abbreviated_type_defs[symmetric] wordarray_length_0_type_def[symmetric] \<Xi>_def[symmetric])
+   apply (frule_tac k = "{D, S}" and K = "[]" in upd.shareable_not_writable(1)[rotated 1]; simp?)
+    apply (rule kindingI; simp?)
+   apply (drule upd.uval_typing_frame; simp?)
+   apply (erule_tac x = ra in allE)
+   apply (erule_tac x = "{}" in allE)
+  apply (rotate_tac -1)
+   apply (erule notE)
+   apply (clarsimp simp: wordarray_fold_no_break_0_type_def abbreviated_type_defs)
+  apply (intro upd.matches_ptrs_some[where r' = "{}" and w' = "{}", simplified]
+      upd.matches_ptrs_empty[where \<tau>s = "[]", simplified])
+   apply (rule upd.u_t_struct; simp?)
+   apply (intro upd.u_t_r_cons1[where r' = "{}" and w' = "{}", simplified] 
+      upd.u_t_prim' upd.u_t_unit upd.u_t_r_empty; simp?)
+    apply (rule upd.u_t_function[OF sum_typecorrect']; (simp add: sum_type_def abbreviated_type_defs subtyping_refl)?)
+   apply (drule upd.type_repr_uval_repr; simp)
+  apply clarsimp
+  apply (rename_tac r'a s'a r' s')
+  apply (erule_tac x = r' in allE)
+  apply (erule_tac x = s' in allE)
+  apply (erule impE, assumption)
+  apply (drule_tac x = "t5_C a' 0 r' FUN_ENUM_sum 0 (unit_t_C 0)" in meta_spec)
+  apply (drule_tac x = 0 in meta_spec)
+  apply clarsimp
+  apply (drule_tac 
+      x = "[mk_urecord [UPtr (ptr_val a') repr, 
+            UPrim (LU32 0), UPrim (LU32 r'),  
+            UFunction Generated_TypeProof.sum [], 
+            UPrim (LU32 0), 
+            UUnit]]" in meta_spec)
+  apply clarsimp
+  apply (drule_tac x = "[option.Some (prod.fst (prod.snd (\<Xi> ''wordarray_fold_no_break_0'')))]" in meta_spec)
+  apply (rename_tac \<sigma>')
+  apply (drule_tac x = \<sigma>' in meta_spec)
+  apply (drule_tac x = s' in meta_spec)
+  apply clarsimp
+  apply (erule impE)
+   apply (elim u_sem_appE u_sem_afunE u_sem_funE u_sem_varE; simp?)
+   apply (erule upd.matches_ptrs_consE; clarsimp)
+   apply (rename_tac ra wa rb wb)
+   apply (drule upd.proc_env_matches_ptrs_abstract[where \<tau>s = "[]", simplified]; simp?,
+      (simp add: \<Xi>_def wordarray_length_0_type_def abbreviated_type_defs)?)
+   apply (clarsimp simp: abbreviated_type_defs[symmetric] wordarray_length_0_type_def[symmetric] \<Xi>_def[symmetric])
+   apply (frule_tac k = "{D, S}" and K = "[]" in upd.shareable_not_writable(1)[rotated 1]; simp?)
+    apply (rule kindingI; simp?)
+   apply (drule upd.uval_typing_frame; simp?)
+   apply (rule_tac x = ra in exI)
+   apply (rule_tac x = "{}" in exI)
+   apply (clarsimp simp: wordarray_fold_no_break_0_type_def abbreviated_type_defs)
+   apply (intro upd.matches_ptrs_some[where r' = "{}" and w' = "{}", simplified]
+      upd.matches_ptrs_empty[where \<tau>s = "[]", simplified])
+   apply (rule upd.u_t_struct; simp?)
+   apply (intro upd.u_t_r_cons1[where r' = "{}" and w' = "{}", simplified] 
+      upd.u_t_prim' upd.u_t_unit upd.u_t_r_empty; simp?)
+    apply (rule upd.u_t_function[OF sum_typecorrect']; (simp add: sum_type_def abbreviated_type_defs subtyping_refl)?)
+   apply (drule upd.type_repr_uval_repr; simp)
+  apply clarsimp
+  apply (erule_tac x = r'a in allE)
+  apply (erule_tac x = s'a in allE)
+  apply clarsimp
+  apply (rename_tac \<sigma>'')
+  apply (intro exI conjI; simp?)
+  apply (elim u_sem_appE u_sem_afunE u_sem_funE; simp)
+  apply clarsimp
+  apply (intro u_sem_let u_sem_var u_sem_afun u_sem_abs_app u_sem_lit u_sem_fun u_sem_unit u_sem_struct; simp?; clarsimp?)
+          apply (rule u_sem_afun)
+         apply (rule u_sem_var[of _ "[_, _]" _ 0, simplified])
+        apply (rule u_sem_lit)
+       apply (rule u_sem_fun)
+      apply (rule u_sem_lit)
+     apply (rule u_sem_unit)
+    apply (rule u_sem_struct)
+    apply (rule u_sem_all_cons, rule u_sem_var)+
+    apply (rule u_sem_all_empty)
+   apply (rule u_sem_afun)
+  apply clarsimp
+  apply (elim u_sem_varE; clarsimp)
+  apply (erule upd.matches_ptrs_consE; clarsimp)
+  apply (drule upd.type_repr_uval_repr; simp)
+  apply (rule u_sem_var[of _ "[_, _, _, _, _, _, _, _]" _ 0, simplified])
+  done
+
+lemma sum_scorres:
+  "valRel \<xi>' v v' \<Longrightarrow> val.scorres (Generated_Shallow_Normal.sum v) (specialise ts Generated_Deep_Normal.sum) [v'] \<xi>'"
+  apply (unfold Generated_Shallow_Normal.sum_def Generated_Deep_Normal.sum_def[simplified])
+  apply (simp only: specialise.simps valRel_records)
+  apply (elim exE conjE)
+  apply (simp only: valRel_unit.simps valRel_u32.simps)
+  apply (intro val.scorres_take val.scorres_var[simplified val.shallow_tac__var_def]
+      scorres_rec_fields[simplified] val.scorres_prim_add; 
+      simp add: valRel_records val.shallow_tac__var_def)
+     apply (fastforce intro: scorres_rec_fields[simplified])+
+  apply (intro val.scorres_prim_add val.scorres_var[simplified val.shallow_tac__var_def];
+      simp add: valRel_records)
+  done
+
+lemma sum_arr_scorres:
+  "\<lbrakk>\<And>i \<gamma> v ts. \<lbrakk>i < length \<gamma>; valRel \<xi>' (v::(32 word) WordArray) (\<gamma> ! i)\<rbrakk>
+    \<Longrightarrow> val.scorres (wordarray_length v) (App (AFun ''wordarray_length'' ts) (Var i)) \<gamma> \<xi>';
+    \<And>i \<gamma> v ts. \<lbrakk>i < length \<gamma>; valRel \<xi>' (v::((32 word) WordArray, 32 word, 32 word,
+      (32 word, 32 word, unit) ElemAO \<Rightarrow> 32 word, 32 word, unit) WordArrayMapP) (\<gamma> ! i);
+      WordArrayMapP.f\<^sub>f v = Generated_Shallow_Normal.sum;
+      \<exists>fs. \<gamma> ! i = VRecord fs \<and> fs ! 3 = (VFunction Generated_Deep_Normal.sum [])\<rbrakk>
+    \<Longrightarrow> val.scorres (wordarray_fold_no_break v) (App (AFun ''wordarray_fold_no_break'' ts) (Var i)) \<gamma> \<xi>';
+    valRel \<xi>' v v'\<rbrakk>
+  \<Longrightarrow> val.scorres (Generated_Shallow_Normal.sum_arr v) (specialise ts Generated_Deep_Normal.sum_arr) [v'] \<xi>'"
+  apply (unfold Generated_Shallow_Normal.sum_arr_def Generated_Deep_Normal.sum_arr_def)
+  apply (simp only: specialise.simps)
+  apply (clarsimp simp: val.scorres_def)
+  apply (erule v_sem_varE)+
+  apply clarsimp
+  apply (drule_tac x = 0 in meta_spec)
+  apply (rename_tac r len)
+  apply (drule_tac x = "[v', v']" in meta_spec)
+  apply (drule_tac x = v in meta_spec)
+  apply (drule_tac x = "[TPrim (Num U32)]" in meta_spec)
+  apply clarsimp
+  apply (erule_tac x = len in allE)
+  apply clarsimp
+  apply (drule_tac x = 0  in meta_spec)
+  apply (drule_tac x = "[VRecord [v', VPrim (LU32 0), VPrim (LU32 (wordarray_length v)), 
+      VFunction Generated_Deep_Normal.sum [], VPrim (LU32 0), VUnit],
+    VUnit, VPrim (LU32 0), VFunction Generated_Deep_Normal.sum [], VPrim (LU32 0),
+    VPrim (LU32 (wordarray_length v)), v', v']" in meta_spec)
+  apply (drule_tac x = "\<lparr>WordArrayMapP.arr\<^sub>f = v, frm\<^sub>f = 0, to\<^sub>f = (wordarray_length v),
+    f\<^sub>f = Generated_Shallow_Normal.sum, acc\<^sub>f = 0, obsv\<^sub>f = ()\<rparr>" in meta_spec)
+  apply (drule_tac x = "[TPrim (Num U32), TPrim (Num U32), TUnit]" in meta_spec)
+  apply clarsimp
+  apply (erule meta_impE)
+   apply (simp add: valRel_records)
+   apply clarsimp
+   apply (cut_tac v' = "VRecord [VPrim (LU32 (ElemAO.elem\<^sub>f x)), VPrim (LU32 (ElemAO.acc\<^sub>f x)), VUnit]"
+      in sum_scorres[where \<xi>' = \<xi>' and ts = "[]", simplified val.scorres_def specialise.simps],
+      (simp add: valRel_records)?)
+   apply (rename_tac s)
+   apply (erule_tac x = s in allE)
+   apply clarsimp
+  apply (erule_tac x = r in allE)
+  apply (clarsimp simp: valRel_records)
+  done
+
+section "The Shallow to C Correspondence With Assumptions"
+
+lemma sum_arr_corres_shallow_C:
+  "\<lbrakk>\<And>i \<gamma> v' \<Gamma>' \<sigma> st.
+    \<lbrakk>i < length \<gamma>; val_rel (\<gamma> ! i) v'; \<Gamma>' ! i = option.Some (prod.fst (prod.snd (\<Xi> ''wordarray_length_0'')))\<rbrakk>
+    \<Longrightarrow> update_sem_init.corres wa_abs_typing_u wa_abs_repr (Generated.state_rel wa_abs_repr)
+         (App (AFun ''wordarray_length_0'' []) (Var i))
+         (do x <- main_pp_inferred.wordarray_length_0' v'; gets (\<lambda>s. x) od)
+         \<xi>1' \<gamma> \<Xi> \<Gamma>' \<sigma> st;
+    \<And>v' i \<gamma> \<Gamma> \<sigma> s.
+    \<lbrakk>t5_C.f_C v' = FUN_ENUM_sum; i < length \<gamma>; val_rel (\<gamma> ! i) v';
+     \<Gamma> ! i = option.Some (prod.fst (prod.snd (\<Xi> ''wordarray_fold_no_break_0'')))\<rbrakk>
+    \<Longrightarrow> update_sem_init.corres wa_abs_typing_u wa_abs_repr (Generated.state_rel wa_abs_repr)
+         (App (AFun ''wordarray_fold_no_break_0'' []) (Var i))
+         (do x <- main_pp_inferred.wordarray_fold_no_break_0' v'; gets (\<lambda>s. x) od)
+         \<xi>1' \<gamma> \<Xi> \<Gamma> \<sigma> s;
+    \<And>i \<gamma> v ts.
+    \<lbrakk>i < length \<gamma>; valRel \<xi>\<^sub>p (v::(32 word) WordArray) (\<gamma> ! i)\<rbrakk>
+    \<Longrightarrow> val.scorres (wordarray_length v) (App (AFun ''wordarray_length'' ts) (Var i)) \<gamma> \<xi>\<^sub>p;
+    \<And>i \<gamma> v ts.
+    \<lbrakk>i < length \<gamma>; valRel \<xi>\<^sub>p (v::((32 word) WordArray, 32 word, 32 word,
+      (32 word, 32 word, unit) ElemAO \<Rightarrow> 32 word, 32 word, unit) WordArrayMapP) (\<gamma> ! i);
+     WordArrayMapP.f\<^sub>f v = Generated_Shallow_Normal.sum;
+     \<exists>fs. \<gamma> ! i = VRecord fs \<and> fs ! 3 = (VFunction Generated_Deep_Normal.sum [])\<rbrakk>
+    \<Longrightarrow> val.scorres (wordarray_fold_no_break v) (App (AFun ''wordarray_fold_no_break'' ts) (Var i)) \<gamma> \<xi>\<^sub>p;
+    value_sem.rename_mono_prog wa_abs_typing_v rename \<Xi> \<xi>\<^sub>m \<xi>\<^sub>p; vv\<^sub>m = value_sem.rename_val rename (value_sem.monoval vv\<^sub>p);
+    correspondence_init.val_rel_shallow_C wa_abs_repr wa_abs_upd_val rename vv\<^sub>s uv\<^sub>C vv\<^sub>p uv\<^sub>m \<xi>\<^sub>p \<sigma> \<Xi>; proc_ctx_wellformed \<Xi>;
+    value_sem.proc_env_matches wa_abs_typing_v \<xi>\<^sub>m \<Xi>;
+    value_sem.matches wa_abs_typing_v \<Xi> [vv\<^sub>m] [option.Some (prod.fst (prod.snd Generated_TypeProof.sum_arr_type))]\<rbrakk>
+    \<Longrightarrow> correspondence_init.corres_shallow_C wa_abs_repr wa_abs_typing_u wa_abs_upd_val rename (Generated.state_rel wa_abs_repr)
+     (Generated_Shallow_Desugar.sum_arr vv\<^sub>s) Generated_TypeProof.sum_arr (main_pp_inferred.sum_arr' uv\<^sub>C) \<xi>1' \<xi>\<^sub>m \<xi>\<^sub>p
+     [uv\<^sub>m] [vv\<^sub>m] \<Xi> [option.Some (prod.fst (prod.snd Generated_TypeProof.sum_arr_type))] \<sigma> s"
+  apply (subgoal_tac "Generated_Shallow_Desugar.sum_arr = Generated_Shallow_Normal.sum_arr")
+   apply (rule corres_shallow_C_intro[OF _ _ _ _ sum_arr_typecorrect',
+        of rename Generated_Deep_Normal.sum_arr vv\<^sub>m vv\<^sub>p _ _ _ _ uv\<^sub>C _ _ _ _ _ vv\<^sub>s]; simp)
+     apply (simp add: Generated_TypeProof.sum_arr_def Generated_Deep_Normal.sum_arr_def)
+     apply (subst rename_def; simp)+
+     apply (simp add: Generated_Deep_Normal.sum_def Generated_TypeProof.sum_def 
+      Generated_TypeProof.abbreviated_type_defs Generated_Deep_Normal.abbreviated_type_defs)
+    apply (rule sum_arr_corres; simp?)
+    apply (drule val_rel_shallow_C_elim; simp)
+   apply (rule sum_arr_scorres[where ts = "[]", simplified])
+     apply (drule val_rel_shallow_C_elim; simp)+
+   apply (clarsimp simp: Generated_Shallow_Desugar.sum_arr_def Generated_Shallow_Normal.sum_arr_def fun_eq_iff)
+   apply (unfold Generated_Shallow_Desugar.sum_def Generated_Shallow_Normal.sum_def)
+   apply simp
+  done
+
+lemma \<xi>1_wordarray_length:
+  "\<xi>1 ''wordarray_length_0'' = upd_wa_length_0"
+  apply (clarsimp simp: fun_eq_iff)
+  done
+
+lemmas wordarray_length_u32_corres = upd_C_wordarray_length_corres_gen[rotated -1, of \<xi>1, OF \<xi>1_wordarray_length]
+
+lemma wordarray_fold_no_break_u32_corres:
+  "\<And>v' i \<gamma> \<Gamma> \<sigma> s.
+    \<lbrakk>t5_C.f_C v' = FUN_ENUM_sum; i < length \<gamma>; val_rel (\<gamma> ! i) v';
+     \<Gamma> ! i = option.Some (prod.fst (prod.snd (\<Xi> ''wordarray_fold_no_break_0'')))\<rbrakk>
+    \<Longrightarrow> corres state_rel (App (AFun ''wordarray_fold_no_break_0'' []) (Var i)) (do x <- wordarray_fold_no_break_0' v';
+                  gets (\<lambda>s. x)
+               od)
+         \<xi>1 \<gamma> \<Xi> \<Gamma> \<sigma> s"
+  thm upd_C_wordarray_fold_no_break_corres_gen
+  apply (subgoal_tac "\<exists>fs. (\<gamma> ! i) = URecord fs")
+   apply (erule exE)
+   apply (rule_tac k = "kinding_fn [] (foldmap_obsv_type ''wordarray_fold_no_break_0'')" and
+      \<xi>0' = \<xi>0 and K' = "[]" and num = U32
+      in upd_C_wordarray_fold_no_break_corres_gen; simp?)
+          apply (rule upd_proc_env_matches_ptrs_\<xi>0_\<Xi>)
+         apply (rule disjI1)
+         apply (clarsimp simp: \<Xi>_def wordarray_fold_no_break_0_type_def)
+        apply (clarsimp simp: \<Xi>_def wordarray_fold_no_break_0_type_def)
+       apply (rule kindingI; simp)
+      apply (clarsimp simp: \<Xi>_def  wordarray_fold_no_break_0_type_def val_rel_simp
+      abbreviated_type_defs cogent_function_val_rel untyped_func_enum_defs)
+    apply (rule typing_app[of _ 
+      "[option.Some (TRecord [(''elem'', TPrim (Num U32), Present),
+        (''acc'', TPrim (Num U32), Present), (''obsv'', TUnit, Present)] Unboxed)]"
+      "[option.Some (TRecord [(''elem'', TPrim (Num U32), Present),
+        (''acc'', TPrim (Num U32), Present), (''obsv'', TUnit, Present)] Unboxed)]"
+      "[option.Some (TRecord [(''elem'', TPrim (Num U32), Present),
+        (''acc'', TPrim (Num U32), Present), (''obsv'', TUnit, Present)] Unboxed)]"
+      _ _
+      "TRecord [(''elem'', TPrim (Num U32), Present), (''acc'', TPrim (Num U32), Present),
+        (''obsv'', TUnit, Present)] Unboxed"] ; simp?)
+      apply (clarsimp simp: split_def)
+      apply (rule_tac k = "{D, S}" in share, rule kindingI; simp?)
+     apply (rule typing_fun; simp?)
+       apply (subst abbreviated_type_defs[symmetric])+
+       apply (subst wordarray_fold_no_break_0_type_def[symmetric])
+       apply (subst \<Xi>_def[symmetric])
+       apply (rule sum_typecorrect'[simplified sum_type_def snd_conv fst_conv])
+      apply (clarsimp simp: empty_def weakening_def)
+      apply (rule_tac k = "{D, S}" in drop, rule kindingI; simp?)
+     apply clarsimp
+    apply (subst abbreviated_type_defs[symmetric])+
+    apply (subst wordarray_fold_no_break_0_type_def[symmetric])
+    apply (subst \<Xi>_def[symmetric])
+    apply (rule typing_var)
+     apply (clarsimp simp: weakening_def empty_def)
+     apply (rule keep)
+     apply (clarsimp simp: abbreviated_type_defs)
+      apply clarsimp
+     apply (clarsimp simp: val_rel_simp cogent_function_val_rel untyped_func_enum_defs)
+     apply (subst dispatch_t4'_def; simp)
+     apply (subst unknown_bind_ignore)
+     apply (simp add: untyped_func_enum_defs)
+     apply (rule corres_app_concrete[simplified]; (simp del: \<xi>0.simps)?)
+     apply (simp add: \<Xi>_def wordarray_fold_no_break_0_type_def del: \<xi>0.simps)
+     apply (subst wordarray_fold_no_break_0_type_def[symmetric])
+     apply (subst \<Xi>_def[symmetric])
+     apply (rule sum_corres[simplified sum_type_def snd_conv fst_conv])
+     apply (clarsimp simp: val_rel_simp)
+    apply (clarsimp simp: fun_eq_iff)
+   apply (clarsimp simp: \<Xi>_def wordarray_fold_no_break_0_type_def abbreviated_type_defs)
+  apply (clarsimp simp: val_rel_simp)
+  done
+
+lemma wordarray_length_u32_scorres:
+  "\<And>i \<gamma> v ts.
+   \<lbrakk>i < length \<gamma>; valRel \<xi>p1 (v::32 word WordArray) (\<gamma> ! i)\<rbrakk> 
+    \<Longrightarrow> val.scorres (wordarray_length v) (App (AFun ''wordarray_length'' ts) (Var i)) \<gamma> \<xi>p1"
+  apply (rule scorres_wordarray_length; clarsimp simp: fun_eq_iff \<xi>p.simps)
+  done
+
+lemma wordarray_fold_no_break_u32_scorres:
+  "\<And>i \<gamma> v ts.
+   \<lbrakk>i < length \<gamma>; valRel \<xi>p1 (v::((32 word) WordArray, 32 word, 32 word,
+      (32 word, 32 word, unit) ElemAO \<Rightarrow> 32 word, 32 word, unit) WordArrayMapP) (\<gamma> ! i);
+    WordArrayMapP.f\<^sub>f v = Generated_Shallow_Normal.sum;
+    \<exists>fs. \<gamma> ! i = VRecord fs \<and> fs ! 3 = VFunction Generated_Deep_Normal.sum []\<rbrakk>
+    \<Longrightarrow> val.scorres (wordarray_fold_no_break v) (App (AFun ''wordarray_fold_no_break'' ts) (Var i)) \<gamma> \<xi>p1"
+  apply (subgoal_tac "\<exists>arr frm to f acc obsv. v = \<lparr>WordArrayMapP.arr\<^sub>f = arr, frm\<^sub>f = frm, to\<^sub>f = to,
+    f\<^sub>f = f, acc\<^sub>f = acc, obsv\<^sub>f = obsv\<rparr>")
+   apply clarsimp
+   apply (rule_tac \<xi>p' = \<xi>p in scorres_wordarray_fold_no_break_u32; simp?)
+  apply (clarsimp simp: fun_eq_iff )
+   apply (clarsimp simp: valRel_records valRel_WordArray_simps)
+   apply (rename_tac x v')
+   apply (cut_tac v = x and ts = "[]" and \<xi>' = \<xi>p and 
+      v' = "VRecord [VPrim (LU32 (ElemAO.elem\<^sub>f x)), VPrim (LU32 (ElemAO.acc\<^sub>f x)), VUnit]" in sum_scorres)
+    apply (clarsimp simp: valRel_records)
+   apply (clarsimp simp: val.scorres_def)
+  apply (clarsimp simp: valRel_records valRel_WordArray_simps)
+  apply (rule_tac x = "WordArrayMapP.arr\<^sub>f v" in exI)
+  apply (rule_tac x = "WordArrayMapP.frm\<^sub>f v" in exI)
+  apply (rule_tac x = "WordArrayMapP.to\<^sub>f v" in exI)
+  apply (rule_tac x = "Generated_Shallow_Normal.sum" in exI)
+  apply (rule_tac x = "WordArrayMapP.acc\<^sub>f v" in exI)
+  apply clarsimp
+  done
+
+section "Putting It All Together"
+
+text
+  "Now with @{thm wordarray_length_u32_corres wordarray_fold_no_break_u32_corres
+   wordarray_length_u32_scorres wordarray_fold_no_break_u32_scorres} we can remove the assumptions
+   about about @{term corres} and @{term val.scorres} for @{term wordarray_length} and
+   @{term wordarray_fold_no_break}."
+
+lemma sum_arr_corres_shallow_C_concrete:
+  "\<lbrakk>value_sem.rename_mono_prog wa_abs_typing_v rename \<Xi> \<xi>m1 \<xi>p1; vv\<^sub>m = value_sem.rename_val rename (value_sem.monoval vv\<^sub>p);
+    correspondence_init.val_rel_shallow_C wa_abs_repr wa_abs_upd_val rename vv\<^sub>s uv\<^sub>C vv\<^sub>p uv\<^sub>m \<xi>p1 \<sigma> \<Xi>; proc_ctx_wellformed \<Xi>;
+    value_sem.proc_env_matches wa_abs_typing_v \<xi>m1 \<Xi>;
+    value_sem.matches wa_abs_typing_v \<Xi> [vv\<^sub>m] [option.Some (prod.fst (prod.snd Generated_TypeProof.sum_arr_type))]\<rbrakk>
+    \<Longrightarrow> correspondence_init.corres_shallow_C wa_abs_repr wa_abs_typing_u wa_abs_upd_val rename (Generated.state_rel wa_abs_repr)
+     (Generated_Shallow_Desugar.sum_arr vv\<^sub>s) Generated_TypeProof.sum_arr (main_pp_inferred.sum_arr' uv\<^sub>C) \<xi>1 \<xi>m1 \<xi>p1
+     [uv\<^sub>m] [vv\<^sub>m] \<Xi> [option.Some (prod.fst (prod.snd Generated_TypeProof.sum_arr_type))] \<sigma> s"
+  apply (rule sum_arr_corres_shallow_C; simp?)
+     apply (rule wordarray_length_u32_corres[simplified]; simp)
+    apply (rule wordarray_fold_no_break_u32_corres[simplified]; simp)
+   apply (rule wordarray_length_u32_scorres; simp)
+  apply (rule wordarray_fold_no_break_u32_scorres; simp)
+  done
+
+section "Further Improvements"
+
+text
+  "We can go one step further by removing the assumptions:
+    * @{term \<open>value_sem.rename_mono_prog wa_abs_typing_v rename \<Xi> \<xi>m1 \<xi>p1\<close>},
+    * @{term \<open>proc_ctx_wellformed \<Xi>\<close>},
+    * @{term \<open>value_sem.proc_env_matches wa_abs_typing_v \<xi>m1 \<Xi>\<close>}.
+
+   The @{term \<open>value_sem.rename_mono_prog\<close>} assumption ensures that  monomorphisation of the whole
+   Cogent program preserves the semantics of abstract functions. With this assumption, we can prove
+   that the monomorphic deep embedding of Cogent expressions refine their polymorphic deep embeddings.
+   We prove this is the case in  @{thm value_sem_rename_mono_prog_rename_\<Xi>_\<xi>m1_\<xi>p1}. Note that the
+   renaming that occurs due to monomorphisation only really affects abstract functions due to their
+   deep embedding being of the form @{term \<open>VAFunction f ts\<close>}, where @{term \<open>(f:: string)\<close>} is the
+   name of the monomorphised abstract function. @{term \<open>value_sem.rename_mono_prog\<close>} is proved
+   by unfolding the definitions of the deep embeddings of the abstract function and case analysis on
+   the arguments and return values. For functions such as @{term wordarray_length}, whose deep
+   embedding is very simple, this proof is very simple. For more complex functions such as
+   @{term wordarray_fold_no_break}, is more tricky due to the fact that
+   @{term wordarray_fold_no_break} is a higher order function, so we need to know that the function
+   it takes as an argument preserves it semantics when monomorphisation. We solve this by first
+   proving @{term \<open>value_sem.rename_mono_prog\<close>} for first order abstract function and then use that
+   result in conjunction with @{thm val.rename_monoexpr_correct} to prove
+   @{term \<open>value_sem.rename_mono_prog\<close>} for second order functions. Note that
+   @{thm val.rename_monoexpr_correct} assumes @{term \<open>proc_ctx_wellformed\<close>} and
+   @{term \<open>value_sem.proc_env_matches\<close>}, which we can prove as described below.
+   We proved @{term \<open>value_sem.rename_mono_prog\<close>} in @{thm value_sem_rename_mono_prog_rename_\<Xi>_\<xi>m_\<xi>p
+   value_sem_rename_mono_prog_rename_\<Xi>_\<xi>m1_\<xi>p1} for first order and second order abstract functions
+   defined in @{term \<xi>m}, @{term \<xi>m1}, @{term \<xi>p} and @{term \<xi>p1}.
+
+   The @{term \<open>proc_ctx_wellformed\<close>} assumption states that the types of our abstract functions
+   are type well-formed. This was fairly easy to prove as it follows from the definition of the
+   types of abstract functions (@{thm proc_ctx_wellformed_\<Xi>}.
+
+   The @{term \<open>value_sem.proc_env_matches\<close>} assumption guarantees the preservation of types for
+   abstract functions. The key theorems @{thm val.mono_correct val.rename_monoexpr_correct}, which
+   are used to prove that the monomorphised Cogent expressions refine their polymorphic counterparts.
+   For abstract functions which are not higher order and do not do any recursion/iteration, it is
+   fairly easy to prove type preservation as this follows from the definition and by using the
+   the @{term val.vval_typing} and @{term val.vval_typing_record} rules. For recursive/iterative
+   functions, this becomes more complex as one would typically need to rely on some sort of
+   invariant. For higher order functions, we need to know that all functions that they could possibly
+   call also preserve typing, however, in our definition of higher order abstract functions, abstract
+   functions can only call first order functions, and we only support up to (and including) second
+   order functions. So we can first prove type preservation for all first order functions, and use
+   this to prove type preservation for higher order functions. We proved
+   @{term \<open>value_sem.proc_env_matches\<close>} in @{thm val_proc_env_matches_\<xi>m_\<Xi>
+   val_proc_env_matches_\<xi>m1_\<Xi>} for first order and second order abstract functions defined in
+   @{term \<xi>m} and @{term \<xi>m1}."
+
+lemmas sum_arr_corres_shallow_C_concrete_strong = 
+  sum_arr_corres_shallow_C_concrete[OF value_sem_rename_mono_prog_rename_\<Xi>_\<xi>m1_\<xi>p1 _ _ 
+                                       proc_ctx_wellformed_\<Xi> val_proc_env_matches_\<xi>m1_\<Xi>]
+
+section "Even More Improvement"
+
+text 
+  "If we look at the definition of @{term corres_shallow_C}, you will notice that we are implicitly
+   assuming that type preservation holds for the deep embedding of abstract functions in the update
+   semantics, abstract functions satisfy the @{term frame} constraints. the the deep embeddings of
+   abstract functions in the update and value semantics correspond, and that the if the deep embedding
+   of an abstract function executes in the update semantics, the corresponding deep embedding in the
+   value semantics will also execute (upward propagation of evaluation). These assumptions are
+   contained in @{term upd.proc_env_matches_ptrs} and @{term proc_env_u_v_matches}.
+
+   Type preservation for abstract functions in the update semantics and @{term frame} constraint
+   satisfiability is contained in @{term upd.proc_env_matches_ptrs}, and can be proved in a similar
+   fashion to proving @{term \<open>value_sem.proc_env_matches\<close>} with the addition of using some lemmas
+   @{term frame} constraints. We proved @{term upd.proc_env_matches_ptrs} in
+   @{thm upd_proc_env_matches_ptrs_\<xi>0_\<Xi> upd_proc_env_matches_ptrs_\<xi>1_\<Xi>} for first order and second
+   order abstract functions defined in @{term \<xi>0} and @{term \<xi>1}.
+  
+   Proving correspondence and upward propagation is contained in @{term proc_env_u_v_matches}.
+   For non higher order functions, we can prove this by unfolding the definitions of the two deep
+   embeddings and use the rules on @{term upd_val_rel} and @{term upd_val_rel_record}. For higher
+   order functions, it is easier to first prove correspondence separately, and use this result to
+   prove upward propagation using the  @{thm val_executes_from_upd_executes}. Note that proving
+   correspondence requires the knowledge that all the deep embeddings of the functions that could be
+   called correspond and upward propagation is true. So we need to first prove 
+   @{term proc_env_u_v_matches} for all the orders below the current and then we can apply the
+   @{thm mono_correspondence} to prove correspondence for the function argument. We proved
+   @{term proc_env_u_v_matches} in @{thm proc_env_u_v_matches_\<xi>0_\<xi>m_\<Xi> proc_env_u_v_matches_\<xi>1_\<xi>m1_\<Xi>}
+   for first order and second order abstract functions defined in @{term \<xi>0}, @{term \<xi>1}, @{term \<xi>m}
+   and @{term \<xi>m1}."
+
+lemma sum_arr_corres_shallow_C_concrete_stronger:
+  "\<lbrakk>vv\<^sub>m = val.rename_val rename (val.monoval vv\<^sub>p); val_rel_shallow_C rename vv\<^sub>s uv\<^sub>C vv\<^sub>p uv\<^sub>m \<xi>p1 \<sigma> \<Xi>;
+    val.matches \<Xi> [val.rename_val rename (val.monoval vv\<^sub>p)] 
+      [option.Some (prod.fst (prod.snd Generated_TypeProof.sum_arr_type))]\<rbrakk>
+    \<Longrightarrow> 
+    (\<sigma>, s) \<in> state_rel \<longrightarrow>
+    (\<exists>r w. u_v_matches \<Xi> \<sigma> [uv\<^sub>m] [val.rename_val rename (val.monoval vv\<^sub>p)]
+            [option.Some (prod.fst (prod.snd Generated_TypeProof.sum_arr_type))] r w) \<longrightarrow>
+    \<not> prod.snd (sum_arr' uv\<^sub>C s) \<and>
+    (\<forall>r' s'.
+        (r', s') \<in> prod.fst (sum_arr' uv\<^sub>C s) \<longrightarrow>
+        (\<exists>\<sigma>' v\<^sub>u\<^sub>m v\<^sub>p.
+            \<xi>1, [uv\<^sub>m] \<turnstile> (\<sigma>, Generated_TypeProof.sum_arr) \<Down>! (\<sigma>', v\<^sub>u\<^sub>m) \<and>
+            \<xi>m1 , [val.rename_val rename
+                    (val.monoval vv\<^sub>p)] \<turnstile> Generated_TypeProof.sum_arr \<Down> val.rename_val rename (val.monoval v\<^sub>p) \<and>
+            (\<sigma>', s') \<in> state_rel \<and> val_rel_shallow_C rename (Generated_Shallow_Desugar.sum_arr vv\<^sub>s) r' v\<^sub>p v\<^sub>u\<^sub>m \<xi>p1 \<sigma>' \<Xi>))"
+  apply (frule sum_arr_corres_shallow_C_concrete_strong[simplified corres_shallow_C_def
+        proc_ctx_wellformed_\<Xi> upd_proc_env_matches_ptrs_\<xi>1_\<Xi> proc_env_u_v_matches_\<xi>1_\<xi>m1_\<Xi>]; simp?)
+  done
+
+term "{(a, b, c) | a b c. \<xi>0 a b c}"
+definition \<xi>_le
+  where "\<xi>_le \<xi>a \<xi>b = ({(a, b, c) | a b c. \<xi>a a b c} \<subseteq> {(a, b, c) | a b c. \<xi>b a b c})"
+
+lemma "\<xi>_le \<xi>0 \<xi>1"
+  apply (clarsimp simp: \<xi>_le_def)
+  apply (drule Meson.imp_to_disjD; clarsimp)
+  apply (drule Meson.imp_to_disjD; clarsimp)
+  apply (erule disjE; clarsimp)
+  apply (drule Meson.imp_to_disjD; clarsimp)
+  apply (drule Meson.imp_to_disjD; clarsimp)
+  apply (drule Meson.imp_to_disjD; clarsimp)
+  apply (erule disjE; clarsimp)
+   apply (intro exI conjI impI; simp)
+  apply (intro exI conjI impI; simp)
+  done
+
+
+lemma "\<xi>_le \<xi>m \<xi>m1"
+  apply (clarsimp simp: \<xi>_le_def)
+  apply (drule Meson.imp_to_disjD; clarsimp)
+  apply (drule Meson.imp_to_disjD; clarsimp)
+  apply (erule disjE; clarsimp)
+  apply (drule Meson.imp_to_disjD; clarsimp)
+  apply (drule Meson.imp_to_disjD; clarsimp)
+  apply (drule Meson.imp_to_disjD; clarsimp)
+  apply (erule disjE; clarsimp)
+   apply (intro exI conjI impI; simp)
+  apply (intro exI conjI impI; simp)
+  done
+
+lemma \<xi>_le_imp: "\<xi>_le \<xi>a \<xi>b \<Longrightarrow> \<xi>a a b c \<longrightarrow> \<xi>b a b c"
+  apply (clarsimp simp: \<xi>_le_def subset_eq)
+  done
+
+lemma "\<lbrakk>\<xi>_le \<xi>a \<xi>b; valRel \<xi>a (a :: 'c \<Rightarrow> 'd) b\<rbrakk> \<Longrightarrow> valRel \<xi>b a b"
+  apply (clarsimp simp: valRel_records)
+  apply (erule disjE; clarsimp)
+  oops
+end (* of context *)
+
+end
